@prefix : <http://www.ciudadpatrimoniomundial.com/ontologias/BCH/> .
@prefix dc: <http://purl.org/dc/elements/1.1/> .
@prefix ns: <http://creativecommons.org/ns#> .
@prefix gml: <http://www.opengis.net/gml/> .
@prefix owl: <http://www.w3.org/2002/07/owl#> .
@prefix rdf: <http://www.w3.org/1999/02/22-rdf-syntax-ns#> .
@prefix xml: <http://www.w3.org/XML/1998/namespace> .
@prefix xsd: <http://www.w3.org/2001/XMLSchema#> .
@prefix bcho: <http://www.ciudadpatrimoniomundial.com/ontologias/BCH/> .
@prefix rdfs: <http://www.w3.org/2000/01/rdf-schema#> .
@prefix skos: <http://www.w3.org/2004/02/skos/core#> .
@prefix cidoc: <http://www.cidoc-crm.org/cidoc-crm/#> .
@prefix terms: <http://purl.org/dc/terms/> .
@prefix mondis: <http://kbss.felk.cvut.cz/ontologies/2011/mondis-core-templates.owl#> .
@prefix bchoData: <http://www.ciudadpatrimoniomundial.com/ontologias/BCH/Data/> .
@prefix mondis: <http://kbss.felk.cvut.cz/ontologies/2011/monument-damage-core.owl#> .
@prefix mondistaxo: <http://kbss.felk.cvut.cz/ontologies/2011/monument-damage-taxonomies.owl#> .
@prefix BldgCitygml2: <http://www.opengis.net/citygml/building/2.0/> .
@base <http://www.ciudadpatrimoniomundial.com/ontologias/BCH/> .


mondis:Agent rdfs:label "M5 Agent"@en.


mondis:CHObject rdfs:label "M1 CH Object"@en.


mondis:Component rdfs:label "M2 Component"@en.

mondis:ComponentManifestationOfDamage rdfs:label "M8 Component Manifesation of Damage"@en.

mondis:Hazard  rdfs:label "M7 Hazard"@en.


mondis:Intervention rdfs:label "M28 Intervention"@en.

mondis:ManifestationOfDamage rdfs:label "M4 ManifestationOfDamage"@en.

mondis:MaterialManifestationOfDamage rdfs:label "M9 Material Manifestation of Damage"@en.

mondis:Risk rdfs:label "M3 Risk"@en.

mondis:Vulnerability rdfs:label "M6 Vulnerability"@en.

mondistaxo:BiologicalColonization rdfs:label "M14 Biological Colonization"@en.

mondistaxo:Crack rdfs:label "M19 Crack"@en.

mondistaxo:DecolorationAndDeposit rdfs:label "M17 Decoloration and Deposit"@en.

mondistaxo:Deformation rdfs:label "M10 Deformation"@en.

mondistaxo:Detachment rdfs:label "M18 Detachment"@en.

mondistaxo:Displacement rdfs:label "M11 Displacement"@en.

mondistaxo:EarthquakeHazard rdfs:label "M24 Eathquake Hazard"@en.

mondistaxo:EarthquakeVulnerability rdfs:label "M20 Eathquake Vulnerability"@en.


mondistaxo:Failure rdfs:label "M13 Failure"@en.

mondistaxo:FireHazard rdfs:label "M25 Fire Hazard"@en.

mondistaxo:FireVulnerability rdfs:label "M21 Fire Vulnerability"@en.

mondistaxo:FloodHazard rdfs:label "M26 Flood Hazard"@en.

mondistaxo:FloodVulnerability rdfs:label "M22 Flood Vulnerability"@en.

mondistaxo:LandslideHazard rdfs:label "M27 Landslide Hazard"@en.
mondistaxo:LandslideVulnerability rdfs:label "M23 Landslide Vulnerability"@en.

mondistaxo:MaterialDeformation rdfs:label "M15 Material Deformation"@en.

mondistaxo:MaterialLoss rdfs:label "M16 Material Loss"@en.

mondistaxo:Rotation rdfs:label "M12 Rotation"@en.


cidoc:E10_Transfer_of_Custody rdfs:label "E10 Transfer of Custody"@en.


cidoc:E11_Modification rdfs:label "E11 Modification"@en.

cidoc:E12_Production rdfs:label "E12 Production"@en.


cidoc:E13_Attribute_Assignment rdfs:label "E13 Attribute Assignment"@en.

cidoc:E14_Condition_Assessment rdfs:label "E14 Condition Assessment"@en.

cidoc:E15_Identifier_Assignment rdfs:label "E15 Identifier Assignment"@en.


cidoc:E17_Type_Assignment rdfs:label "E17 Type Assignment"@en.


cidoc:E18_Physical_Thing rdfs:label "E18 Physical Thing"@en.


cidoc:E19_Physical_Object rdfs:label "E19 Physical Object"@en .


cidoc:E1_CRM_Entity rdfs:label "E1 CRM Entity"@en.


cidoc:E21_Person rdfs:label "E21 Person"@en .


cidoc:E26_Physical_Feature  rdfs:label "E26 Physical Feature"@en .

cidoc:E28_Conceptual_Object rdfs:label "E28 Conceptual Object"@en .

cidoc:E29_Design_or_Procedure rdfs:label "E29 Design or Procedure"@en .

cidoc:E2_Temporal_Entity rdfs:label "E2 Temporal Entity"@en .


cidoc:E39_Actor rdfs:label "E39 Actor"@en.


cidoc:E3_Condition_State rdfs:label "E3 Condition State"@en.


cidoc:E40_Legal_Body rdfs:label "E40 Legal Body"@en.

cidoc:E41_Appellation  rdfs:label "E41 Appellation"@en  .


cidoc:E42_Identifier rdfs:label "E42 Identifier"@en.

cidoc:E44_Place_Appellation rdfs:label "E44 Place Appellation"@en.



cidoc:E45_Address rdfs:label "E45 Address"@en.


cidoc:E46_Section_Definition rdfs:label "E46 Section Definition"@en.


cidoc:E47_Spatial_Coordinates rdfs:label "E47 Spatial Coordinates"@en.

cidoc:E48_Place_Name rdfs:label "E48 Place Name"@en.

cidoc:E49_Time_Appellation rdfs:label "E49 Time Appellation"@en.

cidoc:E4_Period rdfs:label "E4 Period"@en.

cidoc:E50_Date rdfs:label "E50 Date"@en.

cidoc:E51_Contact_Point rdfs:label "E51 Contact Point"@en.


cidoc:E52_Time-Span rdfs:label "E52 Time-Span"@en.


cidoc:E53_Place rdfs:label "E53 Place"@en.


cidoc:E54_Dimension rdfs:label "E54 Dimension"@en.


cidoc:E55_Type rdfs:label "E55 Type"@en.

cidoc:E57_Material rdfs:label "E57 Material"@en.

cidoc:E58_Measurement_Unit rdfs:label "E58 Measurement Unit"@en.

cidoc:E5_Event rdfs:label "E5 Event"@en.

cidoc:E70_Thing rdfs:label "E70 Thing"@en.

cidoc:E71_Man-Made_Thing rdfs:label "E71 Man-Made Thing"@en.


cidoc:E72_Legal_Object rdfs:label "E72 Legal Object"@en.


cidoc:E73_Information_Object rdfs:label "E73 Information Object"@en.

cidoc:E74_Group rdfs:label "E74 Group"@en.

cidoc:E75_Conceptual_Object_Appellation rdfs:label "E75 Conceptual Object Appellation"@en.

cidoc:E77_Persistent_Item rdfs:label "E77 Persistent Item"@en.


cidoc:E79_Part_Addition rdfs:label "E79 Part Addition"@en.

cidoc:E7_Activity rdfs:label "E7 Activity"@en.

cidoc:E80_Part_Removal rdfs:label "E80 Part Removal "@en.

cidoc:E82_Actor_Appellation rdfs:label "E82 Actor Appellation"@en.

cidoc:E89_Propositional_Object rdfs:label "E89 Propositional Object"@en.


cidoc:E90_Symbolic_Object rdfs:label "E90 Symbolic Object"@en.


bcho:HB1_Building rdfs:label "HB1 Building"@en.

bcho:HB2_Geographic_Area rdfs:label "HB2 Geographic Area"@en.

bcho:HB3_Building_Block rdfs:label "HB3 Building Block"@en.

bcho:HB4_Sector rdfs:label "HB4 Sector"@en.

bcho:HB5_Zone rdfs:label "HB5 Zone"@en.

bcho:HB6_City rdfs:label "HB6 City"@en.

bcho:HB7_Component_Type rdfs:label "HB7 Component Type"@en.

bcho:HB8_Facade rdfs:label "HB8 Facade"@en.

bcho:HB9_Structure rdfs:label "HB9 Structure"@en.

bcho:HB10_Roof rdfs:label "HB10 Roof"@en.

bcho:HB11_Arch rdfs:label "HB11 Arch"@en.

bcho:HB12_Balconie rdfs:label "HB12 Balconie"@en.

bcho:HB13_Door rdfs:label "HB13 Door"@en.

bcho:HB14_Protection rdfs:label "HB14 Protection"@en.

bcho:HB15_Window rdfs:label "HB15 Window"@en.

bcho:HB16_Beam rdfs:label "HB16 Beam"@en.

bcho:HB17_BearingWall rdfs:label "HB17 BearingWall"@en.

bcho:HB18_Column rdfs:label "HB18 Column"@en.

bcho:HB19_Mezzanine rdfs:label "HB19 Mezzanine"@en.

bcho:HB20_Stairs rdfs:label "HB20 Stairs"@en.

bcho:HB21_Traditional_Workmanship rdfs:label "HB21 Traditional Workmanship"@en.


bcho:HB22_Tradditional_Workmanship_Assignment rdfs:label "HB22 Tradditional Workmanship Assignment"@en.

bcho:HB23_Scope rdfs:label "HB23 Scope"@en.

bcho:HB24_Level_of_Protection rdfs:label "HB24 Level of Protection"@en.

bcho:HB25_Heritage_Value rdfs:label "HB25 Heritage Value"@en.

bcho:HB26_Heritage_Aspect rdfs:label "HB26 Heritage Aspect"@en.

bcho:HB27_Heritage_Dimension rdfs:label "HB27 Heritage Dimension"@en.

bcho:HB28_Heritage_Feature rdfs:label "HB28 Heritage Feature"@en.

bcho:HB29_Conceptual_Feature rdfs:label "HB29 Conceptual Feature"@en.

bcho:HB30_Building_Physical_Feature rdfs:label "HB30 Building Physical Feature"@en. 

bcho:HB31_Decorative_Elements rdfs:label "HB31 Decorative Elements"@en.

bcho:HB32_Organizational_Aspects rdfs:label "HB32 Organizational Aspects"@en.

bcho:HB33_Type_of_Implantation rdfs:label "HB33 Type of Implantation"@en.

bcho:HB34_Gravity rdfs:label "HB34 Gravity"@en.

bcho:HB35_Gravity_Assignment rdfs:label "HB35 Gravity Assignment"@en.

bcho:HB36_Risk_Assessment rdfs:label "HB36 Risk Assessment"@en.

bcho:HB37_Risk_Assessment_Type rdfs:label "HB37 Risk Assessment Type"@en.

bcho:HB38_Risk_Type rdfs:label "HB38 Risk Type"@en.

bcho:HB39_Vulnerability_Type rdfs:label "HB39 Vulnerability Type"@en.

bcho:HB40_Hazard_Type rdf:type owl:Class ; rdfs:label "HB40 Hazard Type"@en ; rdfs:subClassOf bcho:HB37_Risk_Assessment_Type .

bcho:HB41_Risk_Assignment rdf:type owl:Class ; rdfs:label "HB41 Risk Assignment"@en ; rdfs:subClassOf cidoc:E13_Attribute_Assignment .

bcho:HB42_Vulnerability_Parameter rdf:type owl:Class ; rdfs:label "HB42 Vulnerability Parameter"@en ; rdfs:subClassOf bcho:HB36_Risk_Assessment .

bcho:HB43_Condition_Variable rdf:type owl:Class ; rdfs:label "HB43 Condition Variable"@en ; rdfs:subClassOf cidoc:E3_Condition_State .

bcho:HB44_Condition_Variable_Assignment rdf:type owl:Class ; rdfs:label "HB44 Condition Variable Assignment"@en ; rdfs:subClassOf cidoc:E14_Condition_Assessment .

bcho:HB45_Performance_Status rdfs:label "HB45 Performance Status"@en .

bcho:HB46_Performance_Status_Parameter rdfs:label "HB46 Performance Status Parameter"@en.

bcho:HB47_Performance_Status_Assignment rdfs:label "HB47 Performance Status Assignment"@en.

bcho:HB48_Therapy rdfs:label "HB48 Therapy"@en.

bcho:HB49_Action rdfs:label "HB49 Action"@en.

bcho:HB50_Action_Type rdfs:label "HB50 Action Type"@en.

bcho:HB51_Action_Status rdfs:label "HB51 Action Status"@en.

bcho:HB52_Resource rdfs:label "HB52 Resource"@en.

bcho:HB53_Inspection rdfs:label "HB53 Inspection"@en.

bcho:HB54_Spatial_Representation rdfs:label "HB54 Spatial Representation"@en.

bcho:HB55_Decorative_Supertructure rdfs:label "HB55 Decorative Supertructure"@en .

bcho:HB56_Domain_Type rdfs:label "HB56 Domain Type"@en.

bcho:HB57_Tenure_Type rdfs:label "HB57 Tenure Type"@en.

bcho:HB58_Usage rdfs:label "HB58 Usage"@en.

bcho:HB59_Usage_Asignment rdfs:label "HB59 Usage Asignment"@en.

bcho:HB60_BuildingBlock_Physical_Feature rdfs:label "HB60 BuildingBlock Physical Feature"@en.

bcho:HB61_Building_Usage rdfs:label "HB61 Building Usage"@en.

bcho:HB62_BuildingBlock_Usage rdfs:label "HB62 BuildingBlock Usage"@en.

bcho:HB63_Building_Block_Section rdfs:label "HB63 Building Block Section"@en.

bcho:HB64_Architectural_Style rdfs:label "HB64 Architectural Style"@en.

bcho:HB65_Socio_Economic_Status rdfs:label "HB65 Socio Economic Status"@en.

bcho:HB66_Construction_Permit_Grant rdfs:label "HB66 Construction Permit Grant"@en.



BldgCitygml2:Building rdfs:label "G17 Building"@en.



BldgCitygml2:BuildingFurniture rdfs:label "G33 BuildingFurniture"@en.







BldgCitygml2:BuildingInstallation rdfs:label "G19 Building Installation"@en.



BldgCitygml2:BuildingPart rdfs:label "G18 Building Part"@en.

BldgCitygml2:CeilingSurface rdfs:label "G24 Ceiling Surface"@en.



BldgCitygml2:Door rdfs:label "G31 Door"@en.



BldgCitygml2:FloorSurface rdfs:label "G26 Floor Surface"@en.





BldgCitygml2:GroundSurface rdfs:label "G23 Ground Surface"@en.





BldgCitygml2:IntBuildingInstallation rdfs:label "G34 IntBuildingInstallation"@en.





BldgCitygml2:InteriorWallSurface rdfs:label "G25 Interior Wall Surface"@en.







BldgCitygml2:OuterCeilingSurface rdfs:label "G27 Outer Ceiling Surface"@en.



BldgCitygml2:OuterFloorSurface rdfs:label "G28 Outer Floor Surface"@en.



BldgCitygml2:RoofSurface rdfs:label "G21 Roof Sourface"@en.







BldgCitygml2:Room rdfs:label "G32 Room"@en.



BldgCitygml2:WallSurface rdfs:label "G22 Wall Surface"@en.



BldgCitygml2:Window rdfs:label "G30 Window"@en.







BldgCitygml2:_AbstractBuilding rdfs:label "G16 Abstract Buiding"@en.







BldgCitygml2:_BoundarySurface rdfs:label "G20 Boundary Sourface"@en.



BldgCitygml2:_CityObject rdfs:label "G14 CityObject"@en.



BldgCitygml2:_Opening rdfs:label "G29 Opening"@en.

BldgCitygml2:_Site rdfs:label "G15 Site"@en.



gml:AbstractGeometricAggregate rdfs:label "G3 Abstract Geometric Aggregate"@en.



gml:Curve rdfs:label "G5 Curve"@en.



gml:GeometricPrimitive rdfs:label "G2 GeometricPrimitive"@en.



gml:Geometry rdfs:label "G1 Geometry"@en.



gml:MultiCurve rdfs:label "G10 MultiCurve"@en.



gml:MultiGeometry rdfs:label "G13 MultiGeometry"@en.

gml:MultiPoint rdfs:label "G9 MultiPoint"@en.







gml:MultiSolid rdfs:label "G12 MultiSolid"@en.







gml:MultiSurface rdfs:label "G11 MultiSurface"@en.



gml:Point rdfs:label "G4 Point"@en.







gml:Polygon rdfs:label "G8 Polygon"@en.





gml:Solid rdfs:label "G7 Solid"@en.

gml:Surface rdfs:label "G6 Surface"@en.













mondis:Agent 
rdfs:comment "Carrying factor of a damaging mechanism."@en.

mondis:CHObject 

rdfs:comment "In the context of MONDIS, cultural heritage property refers to any immovable built entity of outstanding universal heritage value (as defined by UNESCO) in the form of both single and complex objects. It includes monuments, buildings and group of buildings, architectonic complexes, sites and infrastructure."@en.

mondis:Component 

rdfs:comment "Element of structural and/or architectural relevance for the physical representation of a c. h. object. Particular components (e.g. construction) coincide with the physical representation of the whole c. h. object while other components might individuate only some of its parts. Components can be organized into a hierarchy of elements accordingly to the scale of analysis required by the user. In this perspective construction can be understood as the 'zero' or 'root' component from which the hierarchy always begins."@en.

mondis:ComponentManifestationOfDamage 
rdfs:comment "Visible or detectable damage on components produced by a damaging mechanism are recorded with the 'M4 Manifestation of Damage' superclass which comprises: 'M8 Component Manifestation of Damage'  and 'M9 MAterial Manifestation of Damage'.
'M8 Component Manifestation of Damage'  comprises: deformations, displacement, rotation, failure and cracks. 
'M9 Material Manifestation of Damage' comprises: biological colonization, material deformation, material loss, decoloration and deposit, detachment and cracks."@en.

mondis:Hazard 
rdfs:comment "The HB36 Risk Assessment superclass represent values of risk, vulnerability and hazard. 
Vulnerability and hazard are subclasified into: Earthquake, Fire, Flood and Landslide.
Vulnerability is also computed usin a set of vulnerability parameters.
Risk is computing considering damages and hazards."@en.

mondis:Intervention 
rdfs:comment "Set of designed procedures aimed at stopping the damaging process and/or its carrying agent and at repairing the manifestation of damage detected on a component. Some of such procedures may aim also (or exclusively) at preventing actions from triggering damaging processes."@en.

mondis:ManifestationOfDamage 
rdfs:comment "Visible or detectable damage on components produced by a damaging mechanism are recorded with the 'M4 Manifestation of Damage' superclass which comprises: 'M8 Component Manifestation of Damage'  and 'M9 MAterial Manifestation of Damage'.
'M8 Component Manifestation of Damage'  comprises: deformations, displacement, rotation, failure and cracks. 
'M9 Material Manifestation of Damage' comprises: biological colonization, material deformation, material loss, decoloration and deposit, detachment and cracks."@en.

mondis:MaterialManifestationOfDamage 
rdfs:comment "Visible or detectable damage on components produced by a damaging mechanism are recorded with the 'M4 Manifestation of Damage' superclass which comprises: 'M8 Component Manifestation of Damage'  and 'M9 MAterial Manifestation of Damage'.
'M8 Component Manifestation of Damage'  comprises: deformations, displacement, rotation, failure and cracks. 
'M9 Material Manifestation of Damage' comprises: biological colonization, material deformation, material loss, decoloration and deposit, detachment and cracks."@en.

mondis:Risk 
rdfs:comment "The HB36 Risk Assessment superclass represent values of risk, vulnerability and hazard. 
Vulnerability and hazard are subclasified into: Earthquake, Fire, Flood and Landslide.
Vulnerability is also computed using a set of vulnerability parameters.
Risk is computing considering damages and hazards."@en.

mondis:Vulnerability 
rdfs:comment "The HB36 Risk Assessment superclass represent values of risk, vulnerability and hazard. 
Vulnerability and hazard are subclasified into: Earthquake, Fire, Flood and Landslide.
Vulnerability is also computed usin a set of vulnerability parameters.
Risk is computing considering damages and hazards."@en.

mondistaxo:BiologicalColonization 
rdfs:comment "'M9 Material Manifestation of Damage' comprises: biological colonization, material deformation, material loss, decoloration and deposit, detachment and cracks."@en.

mondistaxo:Crack 
rdfs:comment "'M8 Component Manifestation of Damage'  comprises: deformations, displacement, rotation, failure and cracks."@en.

mondistaxo:DecolorationAndDeposit 
rdfs:comment "'M9 Material Manifestation of Damage' comprises: biological colonization, material deformation, material loss, decoloration and deposit, detachment and cracks."@en.

mondistaxo:Deformation 
rdfs:comment "'M8 Component Manifestation of Damage'  comprises: deformations, displacement, rotation, failure and cracks."@en.

mondistaxo:Detachment 
rdfs:comment "'M9 Material Manifestation of Damage' comprises: biological colonization, material deformation, material loss, decoloration and deposit, detachment and cracks."@en.

mondistaxo:Displacement 
rdfs:comment "'M8 Component Manifestation of Damage'  comprises: deformations, displacement, rotation, failure and cracks."@en .

mondistaxo:EarthquakeHazard 
rdfs:comment "The HB36 Risk Assessment superclass represent values of risk, vulnerability and hazard. 
Vulnerability and hazard are subclasified into: Earthquake, Fire, Flood and Landslide.
Vulnerability is also computed usin a set of vulnerability parameters.
Risk is computing considering damages and hazards."@en.

mondistaxo:EarthquakeVulnerability 
rdfs:comment "The HB36 Risk Assessment superclass represent values of risk, vulnerability and hazard. 
Vulnerability and hazard are subclasified into: Earthquake, Fire, Flood and Landslide.
Vulnerability is also computed usin a set of vulnerability parameters.
Risk is computing considering damages and hazards."@en.

mondistaxo:Failure 
rdfs:comment "'M8 Component Manifestation of Damage'  comprises: deformations, displacement, rotation, failure and cracks."@en.

mondistaxo:FireHazard 
rdfs:comment "The HB36 Risk Assessment superclass represent values of risk, vulnerability and hazard. 
Vulnerability and hazard are subclasified into: Earthquake, Fire, Flood and Landslide.
Vulnerability is also computed usin a set of vulnerability parameters.
Risk is computing considering damages and hazards."@en.

mondistaxo:FireVulnerability 
rdfs:comment "The HB36 Risk Assessment superclass represent values of risk, vulnerability and hazard. 
Vulnerability and hazard are subclasified into: Earthquake, Fire, Flood and Landslide.
Vulnerability is also computed usin a set of vulnerability parameters.
Risk is computing considering damages and hazards."@en.

mondistaxo:FloodHazard 
rdfs:comment "The HB36 Risk Assessment superclass represent values of risk, vulnerability and hazard. 
Vulnerability and hazard are subclasified into: Earthquake, Fire, Flood and Landslide.
Vulnerability is also computed usin a set of vulnerability parameters.
Risk is computing considering damages and hazards."@en.

mondistaxo:FloodVulnerability 
rdfs:comment "The HB36 Risk Assessment superclass represent values of risk, vulnerability and hazard. 
Vulnerability and hazard are subclasified into: Earthquake, Fire, Flood and Landslide.
Vulnerability is also computed usin a set of vulnerability parameters.
Risk is computing considering damages and hazards."@en.

mondistaxo:LandslideHazard 
rdfs:comment "The HB36 Risk Assessment superclass represent values of risk, vulnerability and hazard. 
Vulnerability and hazard are subclasified into: Earthquake, Fire, Flood and Landslide.
Vulnerability is also computed usin a set of vulnerability parameters.
Risk is computing considering damages and hazards."@en.

mondistaxo:LandslideVulnerability 
rdfs:comment "The HB36 Risk Assessment superclass represent values of risk, vulnerability and hazard. 
Vulnerability and hazard are subclasified into: Earthquake, Fire, Flood and Landslide.
Vulnerability is also computed usin a set of vulnerability parameters.
Risk is computing considering damages and hazards."@en.

mondistaxo:MaterialDeformation 
rdfs:comment "'M9 Material Manifestation of Damage' comprises: biological colonization, material deformation, material loss, decoloration and deposit, detachment and cracks."@en.

mondistaxo:MaterialLoss 
rdfs:comment "'M9 Material Manifestation of Damage' comprises: biological colonization, material deformation, material loss, decoloration and deposit, detachment and cracks."@en.

mondistaxo:Rotation 
rdfs:comment "'M8 Component Manifestation of Damage'  comprises: deformations, displacement, rotation, failure and cracks."@en.








BldgCitygml2:Building
rdfs:comment "The HB1 Building class represent a building conceptually. On the other hand the G17 Building class is employed for the physical representation of a building as a solid, a set or surfaces or foodprints."@en.

BldgCitygml2:BuildingFurniture
rdfs:comment "Type for building furnitures. As subclass of _CityObject, a BuildingFurniture inherits all attributes and relations, in particular an id, names, external references, and generalization relations."@en.


BldgCitygml2:BuildingInstallation
rdfs:comment "A BuildingInstallation is a part of a Building which has not the significance of a BuildingPart. Examples are stairs, antennas, balconies or small roofs. As subclass of _CityObject, a BuildingInstallation inherits all attributes and relations, in particular an id, names, external references, and generalization relations."@en.


BldgCitygml2:BuildingPart
rdfs:comment "Denotes the relation of an _AbstractBuilding to its building parts. The BuildingPart element must either carry a reference to a BuildingPart object or contain a BuildingPart object inline, but neither both nor none."@en.


BldgCitygml2:CeilingSurface 
rdfs:comment "The 'G20 Boundary Surface' class comprises 'G21 Roof Surfaces,' 'G22 Wall Surface,' 'G23 Ground Surface,' 'G24 Ceiling Surface,' 'G25 Interior Wall Surface,' 'G26 Floor Surface,' 'G27 Outer Ceiling Surface,' 'G28 Outer floor surface' classes."@en.

BldgCitygml2:Door
rdfs:comment "Type for doors in boundary surfaces. Used in LOD3 and LOD4 only . As subclass of _CityObject, a Door inherits all attributes and relations, in particular an id, names, external references, and generalization relations."@en.

BldgCitygml2:FloorSurface
rdfs:comment "The 'G20 Boundary Surface' class comprises 'G21 Roof Surfaces,' 'G22 Wall Surface,' 'G23 Ground Surface,' 'G24 Ceiling Surface,' 'G25 Interior Wall Surface,' 'G26 Floor Surface,' 'G27 Outer Ceiling Surface,' 'G28 Outer floor surface' classes."@en.

BldgCitygml2:GroundSurface
rdfs:comment "The 'G20 Boundary Surface' class comprises 'G21 Roof Surfaces,' 'G22 Wall Surface,' 'G23 Ground Surface,' 'G24 Ceiling Surface,' 'G25 Interior Wall Surface,' 'G26 Floor Surface,' 'G27 Outer Ceiling Surface,' 'G28 Outer floor surface' classes."@en. 

BldgCitygml2:IntBuildingInstallation
rdfs:comment "Denotes the relation of an _AbstractBuilding to its interior building installations. The IntBuildingInstallation element must either carry a reference to a IntBuildingInstallation object or contain a IntBuildingInstallation object inline, but neither both nor none. An IntBuildingInstallation is an interior part of a Building which has a specific function or semantical meaning. Examples are interior stairs, railings, radiators or pipes. As subclass of _CityObject, a nIntBuildingInstallation inherits all attributes and relations, in particular an id, names, external references, and generalization relations."@en.

BldgCitygml2:InteriorWallSurface
rdfs:comment "The 'G20 Boundary Surface' class comprises 'G21 Roof Surfaces,' 'G22 Wall Surface,' 'G23 Ground Surface,' 'G24 Ceiling Surface,' 'G25 Interior Wall Surface,' 'G26 Floor Surface,' 'G27 Outer Ceiling Surface,' 'G28 Outer floor surface' classes."@en. 

BldgCitygml2:OuterCeilingSurface
rdfs:comment "The 'G20 Boundary Surface' class comprises 'G21 Roof Surfaces,' 'G22 Wall Surface,' 'G23 Ground Surface,' 'G24 Ceiling Surface,' 'G25 Interior Wall Surface,' 'G26 Floor Surface,' 'G27 Outer Ceiling Surface,' 'G28 Outer floor surface' classes."@en. 

BldgCitygml2:OuterFloorSurface
rdfs:comment "The 'G20 Boundary Surface' class comprises 'G21 Roof Surfaces,' 'G22 Wall Surface,' 'G23 Ground Surface,' 'G24 Ceiling Surface,' 'G25 Interior Wall Surface,' 'G26 Floor Surface,' 'G27 Outer Ceiling Surface,' 'G28 Outer floor surface' classes."@en.

BldgCitygml2:RoofSurface
rdfs:comment "The 'G20 Boundary Surface' class comprises 'G21 Roof Surfaces,' 'G22 Wall Surface,' 'G23 Ground Surface,' 'G24 Ceiling Surface,' 'G25 Interior Wall Surface,' 'G26 Floor Surface,' 'G27 Outer Ceiling Surface,' 'G28 Outer floor surface' classes."@en. 

BldgCitygml2:Room
rdfs:comment "Denotes the relation of an _AbstractBuilding to its rooms. The Room element must either carry a reference to a Room object or contain a Room object inline, but neither both nor none. A Room is a thematic object for modelling the closed parts inside a building. It has to be closed, if necessary by using closure surfaces. The geometry may be either a solid, or a MultiSurface if the boundary is not topologically clean. The room connectivity may be derived by detecting shared thematic openings or closure surfaces: two rooms are connected if both use the same opening object or the same closure surface. The thematic surfaces bounding a room are referenced by the boundedBy property. As subclass of _CityObject, a Room inherits all attributes and relations, in particular an id, names, external references, and generalization relations."@en.

BldgCitygml2:WallSurface
rdfs:comment "The 'G20 Boundary Surface' class comprises 'G21 Roof Surfaces,' 'G22 Wall Surface,' 'G23 Ground Surface,' 'G24 Ceiling Surface,' 'G25 Interior Wall Surface,' 'G26 Floor Surface,' 'G27 Outer Ceiling Surface,' 'G28 Outer floor surface' classes."@en. 

BldgCitygml2:Window
rdfs:comment "Type for windows in boundary surfaces. Used in LOD3 and LOD4 only . As subclass of _CityObject, a window inherits all attributes and relations, in particular an id, names, external references, and generalization relations."@en.

BldgCitygml2:_AbstractBuilding
rdfs:comment "Type describing the thematic and geometric attributes and the associations of buildings. It is an abstract type, only its subclasses Building and BuildingPart can be instantiated. An _AbstractBuilding may consist of BuildingParts, which are again _AbstractBuildings by inheritance. Thus an aggregation hierarchy between _AbstractBuildings of arbitrary depth may be specified. In such an hierarchy, top elements are Buildings, while all other elements are BuildingParts. Each element of such a hierarchy may have all attributes and geometries of _AbstractBuildings. It must, however, be assured than no inconsistencies occur (for example, if the geometry of a Building does not correspond to the geometries of its parts, or if the roof type of a Building is saddle roof, while its parts have an hip roof). As subclass of _CityObject, an _AbstractBuilding inherits all attributes and relations, in particular an id, names, external references, and generalization relations."@en.

BldgCitygml2:_BoundarySurface
rdfs:comment "A BoundarySurface is a thematic object which classifies surfaces bounding an _AbstractBuilding, Room, BuildingInstallation, and IntBuildingInstallation. The geometry of a BoundarySurface is given by MultiSurfaces. As it is a subclass of _CityObject, it inherits all atributes and relations, in particular the external references, and the generalization relations. Denotes the relation of an _AbstractBuilding to its bounding thematic surfaces (walls, roofs, ..). The _BoundarySurface element must either carry a reference to a _BoundarySurface object or contain a _BoundarySurface object inline, but neither both nor none. There is no differentiation between interior surfaces bounding rooms and outer ones bounding buildings (one reason is, that ClosureSurface belongs to both types). It has to be made sure by additional integrity constraints that, e.g. an _AbstractBuilding is not related to CeilingSurfaces or a room not to RoofSurfaces."@en.

BldgCitygml2:_CityObject
rdfs:comment "Type describing the abstract superclass of most CityGML features. Its purpose is to provide a creation and

				a termination date as well as a reference to corresponding objects in other information systems. A generalization relation

				may be used to relate features, which represent the same real-world object in different Levels-of-Detail, i.e. a feature

				and its generalized counterpart(s). The direction of this relation is from the feature to the corresponding generalized

				feature."@en.


BldgCitygml2:_Opening
rdfs:comment "Denotes the relation of an _BondarySurface to its openings (doors, windows). The _Opening element must either carry a reference to an _Opening object or contain an _Opening object inline, but neither both nor none. Type for openings (doors, windows) in boundary surfaces. Used in LOD3 and LOD4 only. As subclass of _CityObject, an _Opening inherits all attributes and relations, in particular an id, names, external references, and generalization relations."@en.


BldgCitygml2:_Site 

rdfs:comment "Type describing the abstract superclass for buildings, facilities, etc. Future extensions of CityGML like

				bridges and tunnels would be modelled as subclasses of _Site. As subclass of _CityObject, a _Site inherits all attributes

				and relations, in particular an id, names, external references, and generalization relations. "@en.

gml:Geometry 


rdfs:comment "In order to represent geometries from the different objects the 'G1 Geometry' class is used. Geometries can be represented by the 'G2 Geometric Primitive' class or the 'G3 Abstract Geometric Aggregate' class."@en. 

gml:AbstractGeometricAggregate

rdfs:comment "In order to represent geometries from the different objects the 'G1 Geometry' class is used. Geometries can be represented by the 'G2 Geometric Primitive' class or the 'G3 Abstract Geometric Aggregate' class. Abstract geometric aggregates are classified into the 'G9 Multipoint,' 'G10 Multicurve,' 'G11 Multisurface,' 'G12 Multisolid,' and 'G13 Multigeometry' classes."@en.

gml:GeometricPrimitive 


rdfs:comment "In order to represent geometries from the different objects the 'G1 Geometry' class is used. Geometries can be represented by the “G2 Geometric Primitive” class or the 'G3 Abstract Geometric Aggregate' class. Geometric primitives are classified into the 'G4 Point,' 'G5 Curve,' 'G6 Surface,' and 'G7 Solid' classes. Surfaces are classified into the 'G8 Polygon' class."@en. 


gml:MultiCurve


rdfs:comment "In order to represent geometries from the different objects the 'G1 Geometry' class is used. Geometries can be represented by the 'G2 Geometric Primitive' class or the 'G3 Abstract Geometric Aggregate' class. Abstract geometric aggregates are classified into the 'G9 Multipoint,' 'G10 Multicurve,' 'G11 Multisurface,' 'G12 Multisolid,' and 'G13 Multigeometry' classes."@en.

gml:MultiGeometry 
rdfs:comment "In order to represent geometries from the different objects the 'G1 Geometry' class is used. Geometries can be represented by the 'G2 Geometric Primitive' class or the 'G3 Abstract Geometric Aggregate' class. Abstract geometric aggregates are classified into the 'G9 Multipoint,' 'G10 Multicurve,' 'G11 Multisurface,' 'G12 Multisolid,' and 'G13 Multigeometry' classes."@en.

gml:MultiPoint 

rdfs:comment "In order to represent geometries from the different objects the 'G1 Geometry' class is used. Geometries can be represented by the 'G2 Geometric Primitive' class or the 'G3 Abstract Geometric Aggregate' class. Abstract geometric aggregates are classified into the 'G9 Multipoint,' 'G10 Multicurve,' 'G11 Multisurface,' 'G12 Multisolid,' and 'G13 Multigeometry' classes."@en.

gml:MultiSolid 

rdfs:comment "In order to represent geometries from the different objects the 'G1 Geometry' class is used. Geometries can be represented by the 'G2 Geometric Primitive' class or the 'G3 Abstract Geometric Aggregate' class. Abstract geometric aggregates are classified into the 'G9 Multipoint,' 'G10 Multicurve,' 'G11 Multisurface,' 'G12 Multisolid,' and 'G13 Multigeometry' classes."@en.

gml:MultiSurface 


rdfs:comment "In order to represent geometries from the different objects the 'G1 Geometry' class is used. Geometries can be represented by the 'G2 Geometric Primitive' class or the 'G3 Abstract Geometric Aggregate' class. Abstract geometric aggregates are classified into the 'G9 Multipoint,' 'G10 Multicurve,' 'G11 Multisurface,' 'G12 Multisolid,' and 'G13 Multigeometry' classes."@en.


gml:Point 
rdfs:comment "In order to represent geometries from the different objects the 'G1 Geometry' class is used. Geometries can be represented by the “G2 Geometric Primitive” class or the 'G3 Abstract Geometric Aggregate' class. Geometric primitives are classified into the 'G4 Point,' 'G5 Curve,' 'G6 Surface,' and 'G7 Solid' classes. Surfaces are classified into the 'G8 Polygon' class."@en. 

gml:Curve 

rdfs:comment "In order to represent geometries from the different objects the 'G1 Geometry' class is used. Geometries can be represented by the “G2 Geometric Primitive” class or the 'G3 Abstract Geometric Aggregate' class. Geometric primitives are classified into the 'G4 Point,' 'G5 Curve,' 'G6 Surface,' and 'G7 Solid' classes. Surfaces are classified into the 'G8 Polygon' class."@en. 

gml:Surface 
rdfs:comment "In order to represent geometries from the different objects the 'G1 Geometry' class is used. Geometries can be represented by the “G2 Geometric Primitive” class or the 'G3 Abstract Geometric Aggregate' class. Geometric primitives are classified into the 'G4 Point,' 'G5 Curve,' 'G6 Surface,' and 'G7 Solid' classes. Surfaces are classified into the 'G8 Polygon' class."@en. 

gml:Solid 
rdfs:comment "In order to represent geometries from the different objects the 'G1 Geometry' class is used. Geometries can be represented by the “G2 Geometric Primitive” class or the 'G3 Abstract Geometric Aggregate' class. Geometric primitives are classified into the 'G4 Point,' 'G5 Curve,' 'G6 Surface,' and 'G7 Solid' classes. Surfaces are classified into the 'G8 Polygon' class."@en. 

gml:Polygon 
rdfs:comment "In order to represent geometries from the different objects the 'G1 Geometry' class is used. Geometries can be represented by the “G2 Geometric Primitive” class or the 'G3 Abstract Geometric Aggregate' class. Geometric primitives are classified into the 'G4 Point,' 'G5 Curve,' 'G6 Surface,' and 'G7 Solid' classes. Surfaces are classified into the 'G8 Polygon' class."@en. 







bcho:HB1_Building
rdfs:comment "The HB1 Building class represent a building conceptually. On the other hand the G17 Building class is employed for the physical representation of a building as a solid, a set or surfaces or foodprints."@en .

bcho:HB2_Geographic_Area
rdfs:comment "In the analysis phase, information regarding heritage entities is collected through the 'M1 CH Object' class. CH objects can be: components, a single building, bigger geographic areas (building blocks, sectors, zones) or the whole city. 

The 'HB2 Geographic Area' class contains the 'HB3 Building Block', 'HB4 Sector' and 'HB5 Zone' subclasses. The city is represented by the 'HB6 City' class."@en.

bcho:HB3_Building_Block
rdfs:comment "The 'HB2 Geographic Area' class contains the 'HB3 Building Block', 'HB4 Sector' and 'HB5 Zone' subclasses. The city is represented by the 'HB6 City' class."@en .

bcho:HB4_Sector
rdfs:comment "The 'HB2 Geographic Area' class contains the 'HB3 Building Block', 'HB4 Sector' and 'HB5 Zone' subclasses. The city is represented by the 'HB6 City' class."@en .

bcho:HB5_Zone
rdfs:comment "The 'HB2 Geographic Area' class contains the 'HB3 Building Block', 'HB4 Sector' and 'HB5 Zone' subclasses. The city is represented by the 'HB6 City' class."@en .

bcho:HB6_City 
rdfs:comment "The 'HB2 Geographic Area' class contains the 'HB3 Building Block', 'HB4 Sector' and 'HB5 Zone' subclasses. The city is represented by the 'HB6 City' class."@en .

bcho:HB7_Component_Type
rdfs:comment "The HB7 Component Type class is a super class which comprises the different types of components such as roofs, facades and structures in general." .

bcho:HB8_Facade
rdfs:comment "The HB8 Facade superclass represents components of this type such as archs, balconies, doors, protections and windows."@en .

bcho:HB9_Structure
rdfs:comment "The HB9 Structure superclass represents components of this type such as beams, bearing walls, columns, mezzaninies and stairs."@en.

bcho:HB10_Roof 
rdfs:comment "The HB10 Roof class represents components of this type."@en.

bcho:HB11_Arch
rdfs:comment "The HB11 Arch class represents components of this type."@en.

bcho:HB12_Balconie
rdfs:comment "The HB12 Balconie class represents components of this type."@en .

bcho:HB13_Door
rdfs:comment "The HB13 Door class represents components of this type."@en.

bcho:HB14_Protection
rdfs:comment "The HB14 Protection class represents components of this type."@en .

bcho:HB15_Window
rdfs:comment "The HB15 Window class represents components of this type."@en.

bcho:HB16_Beam
rdfs:comment "The HB16 Beam class represents components of this type."@en.

bcho:HB17_BearingWall 
rdfs:comment "The HB17 Bearing Wall class represents components of this type."@en.

bcho:HB18_Column
rdfs:comment "The HB18 Column class represents components of this type."@en.

bcho:HB19_Mezzanini
rdfs:comment "The HB19 Mezzanini class represents components of this type."@en.

bcho:HB20_Stairs
rdfs:comment "The HB20 Stairs class represents components of this type."@en.

bcho:HB21_Traditional_Workmanship
rdfs:comment "The HB21 Traditional Workmanship class strores handmade work such as Wooden works, Earth based works, or Special decorative elements."@en.

bcho:HB22_Tradditional_Workmanship_Assignment
rdfs:comment "The HB22 Tradditional Workmanship Assignment class links a CH Object to a Tradditional wormanship."@en .

bcho:HB23_Scope
rdfs:comment "The HB23 Scope class stores the administrative scope on which a protection organism can work. Municipalities for example havea administrative scope which covers the city area."@en.

bcho:HB24_Level_of_Protection
rdfs:comment "The HB24 Level of Protection class sets the level on which a protection organism works; which can be local, national or international. UNESCO for example has an international level of protection whilst municipalities work at local level."@en.

bcho:HB25_Heritage_Value
rdfs:comment "CH Objects have heritage values associated with one or more heritage aspects and dimensions.  Instances of heritage aspects are: Form and design, Materials and substance, Use and function, Tradition, Technique and workmanship, Location and setting, and Spirit and feeling. The heritage dimensions instances are: Artistic, Historic, Social and Scientific. A heritage value is set according several valuable features represented by the 'HB28 Heritage Feature' class."@en.

bcho:HB26_Heritage_Aspect 
rdfs:comment "CH Objects have heritage values associated with one or more heritage aspects and dimensions.  Instances of heritage aspects are: Form and design, Materials and substance, Use and function, Tradition, Technique and workmanship, Location and setting, and Spirit and feeling. The heritage dimensions instances are: Artistic, Historic, Social and Scientific. A heritage value is set according several valuable features represented by the 'HB28 Heritage Feature' class."@en.

bcho:HB27_Heritage_Dimension 
rdfs:comment "CH Objects have heritage values associated with one or more heritage aspects and dimensions.  Instances of heritage aspects are: Form and design, Materials and substance, Use and function, Tradition, Technique and workmanship, Location and setting, and Spirit and feeling. The heritage dimensions instances are: Artistic, Historic, Social and Scientific. A heritage value is set according several valuable features represented by the 'HB28 Heritage Feature' class."@en.

bcho:HB28_Heritage_Feature
rdfs:comment "CH Objects have heritage values that are set according several valuable features represented by the 'HB28 Heritage Feature' class. 
Heritage features can be represented by the 'E26 Physical Feature' or 'HB29 Conceptual Feature' classes. 
The 'E26 Physical Feature' class comprises identifiable features that are physically attached in an integral way to particular physical objects. 
'HB29 Conceptual Feature' class represents immaterial features related to a persistent item."@en.

bcho:HB29_Conceptual_Feature
rdfs:comment "CH Objects have heritage values that are set according several valuable features represented by the 'HB28 Heritage Feature' class. 
Heritage features can be represented by the 'E26 Physical Feature' or 'HB29 Conceptual Feature' classes. 
The 'E26 Physical Feature' class comprises identifiable features that are physically attached in an integral way to particular physical objects. 
'HB29 Conceptual Feature' class represents immaterial features related to a persistent item."@en.

bcho:HB30_Building_Physical_Feature
rdfs:comment "When the heritage unit refers to a building, some physical features are recodered using the 'HB30 Building Physical Feature' superclass which comprises 'HB31 Decorative Element' and 'HB32 Organizational Aspect' classes. 'HB33 Type of implantation' is a subclass of the 'HB32 Organizational Aspect' class. 'PHB2 has courtyard' and 'PHB3 has orchard' properties link the 'HB32 Organizational Aspect' class with its value."@en.

bcho:HB31_Decorative_Elements
rdfs:comment "When the heritage unit refers to a building, some physical features are recodered using the 'HB30 Building Physical Feature' superclass which comprises 'HB31 Decorative Element' and 'HB32 Organizational Aspect' classes. 'HB33 Type of implantation' is a subclass of the 'HB32 Organizational Aspect' class. 'PHB2 has courtyard' and 'PHB3 has orchard' properties link the 'HB32 Organizational Aspect' class with its value."@en.

bcho:HB32_Organizational_Aspects
rdfs:comment "When the heritage unit refers to a building, some physical features are recodered using the 'HB30 Building Physical Feature' superclass which comprises 'HB31 Decorative Element' and 'HB32 Organizational Aspect' classes. 'HB33 Type of implantation' is a subclass of the 'HB32 Organizational Aspect' class. 'PHB2 has courtyard' and 'PHB3 has orchard' properties link the 'HB32 Organizational Aspect' class with its value."@en.

bcho:HB33_Type_of_Implantation
rdfs:comment "When the heritage unit refers to a building, some physical features are recodered using the 'HB30 Building Physical Feature' superclass which comprises 'HB31 Decorative Element' and 'HB32 Organizational Aspect' classes. 'HB33 Type of implantation' is a subclass of the 'HB32 Organizational Aspect' class. 'PHB2 has courtyard' and 'PHB3 has orchard' properties link the 'HB32 Organizational Aspect' class with its value."@en.

bcho:HB34_Gravity
rdfs:comment "Gravity refers to the gravity of deteroration of a heritage value. 
Gravity is computed recording damages (disturbances) and deterioration agents. The 'M4 Manifestation of Damage' class from MONDIS ontology is used to represent damages. Deterioration agents are represesnted using the MONDIS class 'M5 Agent'."@en.

bcho:HB35_Gravity_Assignment
rdfs:comment "The HB35 Gravity Assignment class links a heritage value to a gravity value."@en.


bcho:HB36_Risk_Assessment
rdfs:comment "The HB36 Risk Assessment superclass represent values of risk, vulnerability and hazard. 
Vulnerability and hazard are subclasified into: Earthquake, Fire, Flood and Landslide.
Vulnerability is also computed usin a set of vulnerability parameters.
Risk is computing considering damages and hazards."@en.

bcho:HB37_Risk_Assessment_Type
rdfs:comment "The HB36 Risk Assessment class represent values of risk, vulnerability and hazard. In this regard, the HB37 Risk Assessment Type is a super class which identifies one of this risk assessment classes."@en .

bcho:HB38_Risk_Type
rdfs:comment "The HB36 Risk Assessment class represent values of risk, vulnerability and hazard. Its specific type, in this case is represented by the HB38 Risk Type class."@en.

bcho:HB39_Vulnerability_Type
rdfs:comment "The HB36 Risk Assessment class represent values of risk, vulnerability and hazard. Its specific type, in this case is represented by the HB39 Vulnerability Type class."@en.

bcho:HB40_Hazard_Type
rdfs:comment "The HB36 Risk Assessment class represent values of risk, vulnerability and hazard. Its specific type, in this case is represented by the HB40 Hazard Type class."@en.

bcho:HB41_Risk_Assignment
rdfs:comment "The HB41 Risk Assignment class links a heritage value to a risk."@en.

bcho:HB42_Vulnerability_Parameter
rdfs:comment "The HB36 Risk Assessment superclass represent values of risk, vulnerability and hazard. 
Vulnerability and hazard are subclasified into: Earthquake, Fire, Flood and Landslide.
Vulnerability is also computed usin a set of vulnerability parameters.
Risk is computing considering damages and hazards."@en.

bcho:HB43_Condition_Variable
rdfs:comment "The condition of a building is computing according to several variable conditions such as features of walls, roofs and in general about the constructive system such as:

The relationship between high and thickness of walls
The conexion between walls and roofs
Weather a wall is a bearing wall or a free wall
Presence of damages, dimension and magnitudes
Use of incompatible materials
Among others"@en.

bcho:HB44_Condition_Variable_Assignment
rdfs:comment "A condition variable is composed be the condition itself, a value and a weight. The HB44 Condition Variable Assignment class links the condition variable with its value and weight."@en.

bcho:HB45_Performance_Status
rdfs:comment "In the diagnosis phase a performance status is computed based on the following parameters:
The effect of consequencial damage 
Speed of deterioration: is it stable?			
The relative importance to the significance of the whole ensemble	
Grado de incidencia de la alteracion			
'HBP13 has max limit' and 'HBP14 has min limit' properties establish thresholds for the performance status parameters."@en.

bcho:HB46_Performance_Status_Parameter
rdfs:comment "In the diagnosis phase a performance status is computed based on the following parameters:
The effect of consequencial damage 
Speed of deterioration: is it stable?			
The relative importance to the significance of the whole ensemble	
Grado de incidencia de la alteracion			
'HBP13 has max limit' and 'HBP14 has min limit' properties establish thresholds for the performance status parameters."@en.

bcho:HB47_Performance_Status_Assignment
rdfs:comment "The HB47 Performance Status Assignment class links a heritage value to a performance status."@en.

bcho:HB48_Therapy
rdfs:comment "According to the performance status a therapy with some actions is suggested. The description of the therapy is store in the HB48 Therapy class."@en.

bcho:HB49_Action
rdfs:comment "Actions are sugested during the diagnosis, some of them are implemented in the therapy."@en.


bcho:HB50_Action_Type 
rdfs:comment "Actions are sugested during the diagnosis, some of them are implemented in the therapy. These actions are cathegorized as curative or preventive (direct, indirect). This cathegory is respresented by the HB44 Action Type class."@en.

bcho:HB51_Action_Status 
rdfs:comment "Actions are sugested during the diagnosis, some of them are implemented in the therapy. The HB45 Action Status class determines whether the action was implemented or just suggested."@en.

bcho:HB52_Resource 
rdfs:comment "In order to execute actions some resources are needed. The HB52 Resource class store them."@en.

bcho:HB53_Inspection 
rdfs:comment "The control phase ends with one or more inspections to verify whether the actions reached the conservation objective. The 'HB53 Inspection' class was created for this means."@en.

bcho:HB54_Spatial_Representation
rdfs:comment "The HB54 Spatial Representation superclass comprises the classes from the GENEVA-CityGML classes. The CityGML standard allows the 3D representation of buildings and components."@en.

bcho:HB55_Decorative_Supertructure 
rdfs:comment "The HB55 Decorative Supertructure superclass represent decorative architectural elements such as cornices, pilasters, tarraves, etc."@en.


cidoc:E1_CRM_Entity
rdfs:comment "Scope note:	
This class comprises all things in the universe of discourse of the CIDOC Conceptual Reference Model. 

It is an abstract concept providing for three general properties:
1.Identification by name or appellation, and in particular by a preferred identifier
2.Classification by type, allowing further refinement of the specific subclass an instance belongs to 
3.Attachment of free text for the expression of anything not captured by formal properties

With the exception of E59 Primitive Value, all other classes within the CRM are directly or indirectly specialisations of E1 CRM Entity. 

Examples:
the earthquake in Lisbon 1755 (E5)

In First Order Logic: 
E1(x)"@en .

cidoc:E2_Temporal_Entity
rdfs:comment "Scope note:
This class comprises all phenomena, such as the instances of E4 Periods, E5 Events and states, which happen over a limited extent in time. This extent in time must be contiguous, i.e., without gaps. In case the defining kinds of phenomena for an instance of E2 Temporal Entity cease to happen, and occur later again at another time, we regard that the former E2 Temporal Entity has ended and a new instance has come into existence. In more intuitive terms, the same event cannot happen twice.

In some contexts, these are also called perdurants. This class is disjoint from E77 Persistent Item. This is an abstract class and has no direct instances. E2 Temporal Entity is specialized into E4 Period, which applies to a particular geographic area (defined with a greater or lesser degree of precision), and E3 Condition State, which applies to instances of E18 Physical Thing.

Examples:
- Bronze Age (E4)
- the earthquake in Lisbon 1755 (E5)
- the Peterhof Palace near Saint Petersburg being in ruins from 1944 – 1946 (E3)

In First Order Logic:
E2(x) ⊃ E1(x)"@en .



cidoc:E3_Condition_State
rdfs:comment "Scope note:
This class comprises the states of objects characterised by a certain condition over a time-span.

An instance of this class describes the prevailing physical condition of any material object or
feature during a specific E52 Time Span. In general, the time-span for which a certain
condition can be asserted may be shorter than the real time-span, for which this condition held.
The nature of that condition can be described using  P2 has type. For example, the E3
Condition State \"condition of the SS Great Britain between 22 September 1846 and 27 August
1847\" can be characterized as E55 Type \"wrecked\".

Examples:
- the \"Amber Room\" in Tsarskoje Selo being completely reconstructed from summer 2003 until now
- the Peterhof Palace near Saint Petersburg being in ruins from 1944 – 1946
- the state of my turkey in the oven at 14:30 on 25 December, 2002 (P2 has type: E55 Type \"still not cooked\")

In First Order Logic:
E3(x) ⊃ E2(x)"@en .


cidoc:E4_Period
rdfs:comment "Scope note:
This class comprises sets of coherent phenomena or cultural manifestations occurring in time and space.

It is the social or physical coherence of these phenomena that identify an E4 Period and not the associated spatiotemporal extent. This extent is only the 'ground' or space in an abstract physical sense that the actual process of growth, spread and retreat has covered. Consequently, different periods can overlap and coexist in time and space, such as when a nomadic culture exists in the same area and time as a sedentary culture. This also means that overlapping land use rights, common among first nations, amounts to overlapping periods.

Often, this class is used to describe prehistoric or historic periods such as the 'Neolithic Period', the 'Ming Dynasty' or the 'McCarthy Era', but also geopolitical units and activities of settlements are regarded as special cases of E4 Period. However, there are no assumptions about the scale of the associated phenomena. In particular all events are seen as synthetic processes consisting of coherent phenomena. Therefore E4 Period is a superclass of E5 Event. For example, a modern clinical E67 Birth can be seen as both an atomic E5 Event and as an E4 Period that consists of multiple activities performed by multiple instances of E39 Actor.

As the actual extent of an E4 Period in spacetime we regard the trajectories of the participating physical things during their participation in an instance of E4 Period. This includes the open spaces via which these things have interacted and the spaces by which they had the potential to interact during that period or event in the way defined by the type of the respective period or event. Examples include the air in a meeting room transferring the voices of the participants. Since these phenomena are fuzzy, we assume the spatiotemporal extent to be contiguous, except for cases of phenomena spreading out over islands or other separated areas, including geopolitical units distributed over disconnected areas such as islands or colonies.

Whether the trajectories necessary for participants to travel between these areas are regarded as part of the spatiotemporal extent or not has to be decided in each case based on a concrete analysis, taking use of the sea for other purposes than travel, such as fishing, into consideration. One may also argue that the activities to govern disconnected areas imply travelling through spaces connecting them and that these areas hence are spatially connected in a way, but it appears counterintuitive to consider for instance travel routes in international waters as extensions of geopolitical units.

Consequently, an instance of E4 Period may occupy a number of disjoint spacetime volumes, however there must not be a discontinuity in the timespan covered by these spacetime volumes. This means that an instance of E4 Period must be contiguous in time. If it has ended in all areas, it has ended as a whole. However it may end in one area before another, such as in the Polynesian migration, and it continues as long as it is ongoing in at least one area.

We model E4 Period as a subclass of E2 Temporal Entity and of E92 Spacetime volume. The latter is intended as a phenomenal spacetime volume as defined in CRMgeo (Doerr and Hiebel 2013). By virtue of this multiple inheritance we can discuss the physical extent of an E4 Period without representing each instance of it together with an instance of its associated spacetime volume. This model combines two quite different kinds of substance: an instance of E4 Period is a phenomena while a spacetime volume is an aggregation of points in spacetime. However, the real spatiotemporal extent of an instance of E4 Period is regarded to be unique to it due to all its details and fuzziness; its identity and existence depends uniquely on the identity of the instance of E4 Period. Therefore this multiple inheritance is unambiguous and effective and furthermore corresponds to the intuitions of natural language.

There are two different conceptualisations of ‘artistic style’, defined either by physical features or by historical context. For example, 'Impressionism' can be viewed as a period lasting from approximately 1870 to 1905 during which paintings with particular characteristics were produced by a group of artists that included (among others) Monet, Renoir, Pissarro, Sisley and Degas. Alternatively, it can be regarded as a style applicable to all paintings sharing the characteristics of the works produced by the Impressionist painters, regardless of historical context. The first interpretation is an instance of E4 Period, and the second defines morphological object types that fall under E55 Type.

Another specific case of an E4 Period is the set of activities and phenomena associated with a settlement, such as the populated period of Nineveh.

Examples:
Jurassic
European Bronze Age
Italian Renaissance
Thirty Years War
Sturm und Drang
Cubism

In First Order Logic: 
E4(x) ⊃ E2(x)
E4(x) ⊃ E92(x)"@en .


cidoc:E5_Event
rdfs:comment "Scope note:
This class comprises changes of states in cultural, social or physical systems, regardless of scale, brought about by a series or group of coherent physical, cultural, technological or legal phenomena. Such changes of state will affect instances of E77 Persistent Item or its subclasses.

The distinction between an E5 Event and an E4 Period is partly a question of the scale of observation. Viewed at a coarse level of detail, an E5 Event is an 'instantaneous' change of state. At a fine level, the E5 Event can be analysed into its component phenomena within a space and time frame, and as such can be seen as an E4 Period. The reverse is not necessarily the case: not all instances of E4 Period give rise to a noteworthy change of state.

Examples:
- the birth of Cleopatra (E67)
- the destruction of Herculaneum by volcanic eruption in 79 AD (E6)
- World War II (E7)
- the Battle of Stalingrad (E7)
- the Yalta Conference (E7)
- my birthday celebration 28-6-1995 (E7)
- the falling of a tile from my roof last Sunday
- the CIDOC Conference 2003 (E7)

In First Order Logic:
E5(x) ⊃ E4(x)"@en .


cidoc:E7_Activity
rdfs:comment "Scope note:
This class comprises actions intentionally carried out by instances of E39 Actor that result in changes of state in the cultural, social, or physical systems documented.

This notion includes complex, composite and long-lasting actions such as the building of a settlement or a war, as well as simple, short-lived actions such as the opening of a door.

Examples:
- the Battle of Stalingrad
- the Yalta Conference
- my birthday celebration 28-6-1995
- the writing of \"Faust\" by Goethe (E65)
- the formation of the Bauhaus 1919 (E66)
- calling the place identified by TGN '7017998' 'Quyunjig' by the people of Iraq
- Kira Weber working in glass art from 1984 to 1993
- Kira Weber working in oil and pastel painting from 1993

In First Order Logic:
E7(x) ⊃ E5(x)"@en .

cidoc:E10_Transfer_of_Custody

rdfs:comment "This class comprises transfers of physical custody of objects between instances of E39 Actor. 
The recording of the donor and/or recipient is optional. It is possible that in an instance of E10 Transfer of Custody there is either no donor or no recipient. Depending on the circumstances it may describe:
1.	the beginning of custody 
2.	the end of custody 
3.	the transfer of custody 
4.	the receipt of custody from an unknown source
5.	the declared loss of an object
The distinction between the legal responsibility for custody and the actual physical possession of the object should be expressed using the property P2 has type (is type of). A specific case of transfer of custody is theft.
The interpretation of the museum notion of \"accession\" differs between institutions. The CRM therefore models legal ownership and physical custody separately. Institutions will then model their specific notions of accession and deaccession as combinations of these.
"@en .

cidoc:E11_Modification


rdfs:comment "This class comprises all instances of E7 Activity that create, alter or change E24 Physical Man-Made Thing. 
This class includes the production of an item from raw materials, and other so far undocumented objects, and the preventive treatment or restoration of an object for conservation. 
Since the distinction between modification and production is not always clear, modification is regarded as the more generally applicable concept. This implies that some items may be consumed or destroyed in a Modification, and that others may be produced as a result of it. An event should also be documented using E81 Transformation if it results in the destruction of one or more objects and the simultaneous production of others using parts or material from the originals. In this case, the new items have separate identities. 
If the instance of the E29 Design or Procedure utilized for the modification prescribes the use of specific materials, they should be documented using property P68 foresees use of (use foreseen by): E57 Material of E29 Design or Procedure, rather than via P126 employed (was employed in): E57 Material.
"@en .

cidoc:E12_Production


rdfs:comment "This class comprises activities that are designed to, and succeed in, creating one or more new items. 
It specializes the notion of modification into production. The decision as to whether or not an object is regarded as new is context sensitive. Normally, items are considered “new” if there is no obvious overall similarity between them and the consumed items and material used in their production. In other cases, an item is considered “new” because it becomes relevant to documentation by a modification. For example, the scribbling of a name on a potsherd may make it a voting token. The original potsherd may not be worth documenting, in contrast to the inscribed one. 
This entity can be collective: the printing of a thousand books, for example, would normally be considered a single event. 
An event should also be documented using E81 Transformation if it results in the destruction of one or more objects and the simultaneous production of others using parts or material from the originals. In this case, the new items have separate identities and matter is preserved, but identity is not.
"@en .

cidoc:E13_Attribute_Assignment
rdfs:comment "Scope note:
This class comprises the actions of making assertions about properties of an object or any relation between two items or concepts.

This class allows the documentation of how the respective assignment came about, and whose opinion it was. All the attributes or properties assigned in such an action can also be seen as directly attached to the respective item or concept, possibly as a collection of contradictory values. All cases of properties in this model that are also described indirectly through an action are characterised as \"short cuts\" of this action. This redundant modelling of two alternative views is preferred because many implementations may have good reasons to model either the action or the short cut, and the relation between both alternatives can be captured by simple rules.

In particular, the class describes the actions of people making propositions and statements during certain museum procedures, e.g. the person and date when a condition statement was made, an identifier was assigned, the museum object was measured, etc. Which kinds of such assignments and statements need to be documented explicitly in structures of a schema rather than free text, depends on if this information should be accessible by structured queries.

Examples:
- the assessment of the current ownership of Martin Doerr's silver cup in February 1997

In First Order Logic: 
E13(x) ⊃ E7(x)"@en .

cidoc:E14_Condition_Assessment
rdfs:comment "Scope note:
This class describes the act of assessing the state of preservation of an object during a particular period.

The condition assessment may be carried out by inspection, measurement or through historical research. This class is used to document circumstances of the respective assessment that may be relevant to interpret its quality at a later stage, or to continue research on related documents.

Examples:
- last year's inspection of humidity damage to the frescos in the St. George chapel in our village

In First Order Logic:
E14(x) ⊃ E13(x)"@en .

cidoc:E15_Identifier_Assignment
rdfs:comment "Scope note:
This class comprises activities that result in the allocation of an identifier to an instance of E1 CRM Entity. An E15 Identifier Assignment may include the creation of the identifier from multiple constituents, which themselves may be instances of E41 Appellation. The syntax and kinds of constituents to be used may be declared in a rule constituting an instance of E29 Design or Procedure.

Examples of such identifiers include Find Numbers, Inventory Numbers, uniform titles in the sense of librarianship and Digital Object Identifiers (DOI). Documenting the act of identifier assignment and deassignment is especially useful when objects change custody or the identification system of an organization is changed. In order to keep track of the identity of things in such cases, it is important to document by whom, when and for what purpose an identifier is assigned to an item.

The fact that an identifier is a preferred one for an organisation can be expressed by using the property E1 CRM Entity. P48 has preferred identifier (is preferred identifier of): E42 Identifier. It can better be expressed in a context independent form by assigning a suitable E55 Type, such as \"preferred identifier assignment\", to the respective instance of E15 Identifier Assignment via the P2 has type property.

Examples:
- Replacement of the inventory number TA959a by GE34604 for a 17th century lament cloth at the Museum Benaki, Athens
- Assigning the author-uniform title heading \"Goethe, Johann Wolfgang von, 1749-1832. Faust. 1. Theil.\" for a work (E28)
- On June 1, 2001 assigning the personal name heading \"Guillaume, de Machaut, ca. 1300-1377\" (E42,E82) to Guillaume de Machaut (E21)

In First Order Logic:
E15(x) ⊃ E13(x)"@en .

cidoc:E16_Measurement
rdfs:comment "Scope note:
This class comprises actions measuring physical properties and other values that can be determined by a systematic procedure.

Examples include measuring the monetary value of a collection of coins or the running time of a specific video cassette.

The E16 Measurement may use simple counting or tools, such as yardsticks or radiation detection devices. The interest is in the method and care applied, so that the reliability of the result may be judged at a later stage, or research continued on the associated documents. The date of the event is important for dimensions, which may change value over time, such as the length of an object subject to shrinkage. Details of methods and devices are best handled as free text, whereas basic techniques such as \"carbon 14 dating\" should be encoded using P2 has type (is type of:) E55 Type.

Examples:
- measurement of height of silver cup 232 on the 31st August 1997
- the carbon 14 dating of the \"Schoeninger Speer II\" in 1996 [an about 400.000 years old Palaeolithic complete wooden spear found in Schoeningen, Niedersachsen, Germany in 1995]

In First Order Logic:
E16(x) ⊃ E13(x)"@en .

cidoc:E17_Type_Assignment
rdfs:comment "Scope note:
This class comprises the actions of classifying items of whatever kind. Such items include objects, specimens, people, actions and concepts.

This class allows for the documentation of the context of classification acts in cases where the value of the classification depends on the personal opinion of the classifier, and the date that the classification was made. This class also encompasses the notion of \"determination\", i.e. the systematic and molecular identification of a specimen in biology.

Examples:
- the first classification of object GE34604 as Lament Cloth, October 2nd
- the determination of a cactus in Martin Doerr's garden as 'Cereus hildmannianus K.Schumann', July 2003

In First Order Logic:
E17(x) ⊃ E13(x)"@en .

cidoc:E18_Physical_Thing
rdfs:comment "Scope note:
This class comprises all persistent physical items with a relatively stable form, man-made or natural.

Depending on the existence of natural boundaries of such things, the CRM distinguishes the instances of E19 Physical Object from instances of E26 Physical Feature, such as holes, rivers, pieces of land etc. Most instances of E19 Physical Object can be moved (if not too heavy), whereas features are integral to the surrounding matter.

An instance of E18 Physical Thing occupies not only a particular geometric space, but in the course of its existence it also forms a trajectory through spacetime, which occupies a real, that is phenomenal, volume in spacetime. We include in the occupied space the space filled by the matter of the physical thing and all its inner spaces, such as the interior of a box. Physical things consisting of aggregations of physically unconnected objects, such as a set of chessmen, occupy a number of individually contiguous spacetime volumes equal to the number of unconnected objects that constitute the set.

We model E18 Physical Thing to be a subclass of E72 Legal Object and of E92 Spacetime volume. The latter is intended as a phenomenal spacetime volume as defined in CRMgeo (Doerr and Hiebel 2013). By virtue of this multiple inheritance we can discuss the physical extent of an E18 Physical Thing without representing each instance of it together with an instance of its associated spacetime volume. This model combines two quite different kinds of substance: an instance of E18 Physical Thing is matter while a spacetime volume is an aggregation of points in spacetime. However, the real spatiotemporal extent of an instance of E18 Physical Thing is regarded to be unique to it, due to all its details and fuzziness; its identity and existence depends uniquely on the identity of the instance of E18 Physical Thing. Therefore this multiple inheritance is unambiguous and effective and furthermore corresponds to the intuitions of natural language.

The CIDOC CRM is generally not concerned with amounts of matter in fluid or gaseous states.

Examples:
- the Cullinan Diamond (E19)
- the cave \"Ideon Andron\" in Crete (E26)
- the Mona Lisa (E22)

In First Order Logic:
E18(x) ⊃ E72(x)
E18(x) ⊃ E92(x)"@en .

cidoc:E19_Physical_Object
rdfs:comment "Scope note:
This class comprises items of a material nature that are units for documentation and have physical boundaries that separate them completely in an objective way from other objects.

The class also includes all aggregates of objects made for functional purposes of whatever kind, independent of physical coherence, such as a set of chessmen. Typically, instances of E19 Physical Object can be moved (if not too heavy).

In some contexts, such objects, except for aggregates, are also called \"bona fide objects\" (Smith & Varzi, 2000, pp.401-420), i.e. naturally defined objects.

The decision as to what is documented as a complete item, rather than by its parts or components, may be a purely administrative decision or may be a result of the order in which the item was acquired.

Examples:
- John Smith
- Aphrodite of Milos
- the Palace of Knossos
- the Cullinan diamond
- Apollo 13 at the time of launch

In First Order Logic:
E19(x) ⊃ E18(x)"@en .



cidoc:E21_Person
rdfs:comment "Scope note:
This class comprises real persons who live or are assumed to have lived.

Legendary figures that may have existed, such as Ulysses and King Arthur, fall into this class if the documentation refers to them as historical figures. In cases where doubt exists as to whether several persons are in fact identical, multiple instances can be created and linked to indicate their relationship. The CRM does not propose a specific form to support reasoning about possible identity.

Examples:
- Tut-Ankh-Amun
- Nelson Mandela

In First Order Logic:
E21(x) ⊃ E20(x)
E21(x) ⊃ E39(x)"@en .

cidoc:E26_Physical_Feature
rdfs:comment "Scope note:
This class comprises identifiable features that are physically attached in an integral way to particular physical objects.

Instances of E26 Physical Feature share many of the attributes of instances of E19 Physical Object. They may have a one-, two- or three-dimensional geometric extent, but there are no natural borders that separate them completely in an objective way from the carrier objects. For example, a doorway is a feature but the door itself, being attached by hinges, is not.

Instances of E26 Physical Feature can be features in a narrower sense, such as scratches, holes, reliefs, surface colours, reflection zones in an opal crystal or a density change in a piece of wood. In the wider sense, they are portions of particular objects with partially imaginary borders, such as the core of the Earth, an area of property on the surface of the Earth, a landscape or the head of a contiguous marble statue. They can be measured and dated, and it is sometimes possible to state who or what is or was responsible for them. They cannot be separated from the carrier object, but a segment of the carrier object may be identified (or sometimes removed) carrying the complete feature.

This definition coincides with the definition of \"fiat objects\" (Smith & Varzi, 2000, pp.401-420), with the exception of aggregates of \"bona fide objects\".

Examples:
- the temple in Abu Simbel before its removal, which was carved out of solid rock
- Albrecht Duerer's signature on his painting of Charles the Great
- the damage to the nose of the Great Sphinx in Giza
- Michael Jackson's nose prior to plastic surgery

In First Order Logic:
E26(x) ⊃ E18(x)"@en .

cidoc:E28_Conceptual_Object
rdfs:comment "Scope note:
This class comprises non-material products of our minds and other human produced data that have become objects of a discourse about their identity, circumstances of creation or historical implication. The production of such information may have been supported by the use of technical devices such as cameras or computers.

Characteristically, instances of this class are created, invented or thought by someone, and then may be documented or communicated between persons. Instances of E28 Conceptual Object have the ability to exist on more than one particular carrier at the same time, such as paper, electronic signals, marks, audio media, paintings, photos, human memories, etc.
They cannot be destroyed. They exist as long as they can be found on at least one carrier or in at least one human memory. Their existence ends when the last carrier and the last memory are lost.

Examples:
- Beethoven's \"Ode an die Freude\" (Ode to Joy) (E73)
- the definition of \"ontology\" in the Oxford English Dictionary
- the knowledge about the victory at Marathon carried by the famous runner
- 'Maxwell equations' [preferred subject access point from LCSH,
 http://lccn.loc.gov/sh85082387, as of 19 November 2012]
- 'Equations, Maxwell' [variant subject access point, from the same source]

In First Order Logic:
E28(x) ⊃ E71(x)"@en .

cidoc:E29_Design_or_Procedure
rdfs:comment "Scope note:
This class comprises documented plans for the execution of actions in order to achieve a result of a specific quality, form or contents. In particular it comprises plans for deliberate human activities that may result in the modification or production of instances of E24 Physical Thing.

Instances of E29 Design or Procedure can be structured in parts and sequences or depend on others. This is modelled using P69 has association with (is associated with)..

Designs or procedures can be seen as one of the following:

1. A schema for the activities it describes
2. A schema of the products that result from their application.
3. An independent intellectual product that may have never been applied, such as Leonardo da Vinci's famous plans for flying machines.

Because designs or procedures may never be applied or only partially executed, the CRM models a loose relationship between the plan and the respective product.

Examples:
- the ISO standardisation procedure
- the musical notation of Beethoven's \"Ode to Joy\"
- the architectural drawings for the Kölner Dom in Cologne, Germany
- The drawing on the folio 860 of the Codex Atlanticus from Leonardo da Vinci, 1486-1490, kept in the Biblioteca Ambrosiana in Milan

In First Order Logic:
E29(x) ⊃ E73(x)"@en .


cidoc:E39_Actor
rdfs:comment "Scope note:
This class comprises people, either individually or in groups, who have the potential to perform intentional actions of kinds for which someone may be held responsible.

The CRM does not attempt to model the inadvertent actions of such actors. Individual people should be documented as instances of E21 Person, whereas groups should be documented as instances of either E74 Group or its subclass E40 Legal Body.

Examples:
- London and Continental Railways (E40)
- the Governor of the Bank of England in 1975 (E21)
- Sir Ian McKellan (E21)

In First Order Logic:
E39(x) ⊃ E77(x)"@en .


cidoc:E40_Legal_Body
rdfs:comment "Scope note:
This class comprises institutions or groups of people that have obtained a legal recognition as a group and can act collectively as agents.

This means that they can perform actions, own property, create or destroy things and can be held collectively responsible for their actions like individual people. The term 'personne morale' is often used for this in French.

Examples:
- Greenpeace
- Paveprime Ltd
- the National Museum of Denmark

In First Order Logic:
E40(x) ⊃ E74(x)"@en .

cidoc:E41_Appellation
rdfs:comment "Scope note:
This class comprises signs, either meaningful or not, or arrangements of signs following a specific syntax, that are used or can be used to refer to and identify a specific instance of some class or category within a certain context. 

Instances of E41 Appellation do not identify things by their meaning, even if they happen to have one, but instead by convention, tradition, or agreement. Instances of E41 Appellation are cultural constructs; as such, they have a context, a history, and a use in time and space by some group of users. A given instance of E41 Appellation can have alternative forms, i.e., other instances of E41 Appellation that are always regarded as equivalent independent from the thing it denotes. 

Specific subclasses of E41 Appellation should be used when instances of E41 Appellation of a characteristic form are used for particular objects. Instances of E49 Time Appellation, for example, which take the form of instances of E50 Date, can be easily recognised.

E41 Appellation should not be confused with the act of naming something. Cf. E15 Identifier Assignment 

Examples:
- \"Martin\" 
- \"the Forth Bridge\"
- \"the Merchant of Venice\" (E35)
- \"Spigelia marilandica (L.) L.\" [not the species, just the name]
- \"information science\" [not the science itself, but the name through which we refer to it in an English-speaking context] 
- '安' [Chinese \"an\", meaning \"peace\"]

In First Order Logic:
E41(x) ⊃ E90(x)"@en .

cidoc:E42_Identifier
rdfs:comment "Scope note:
This class comprises strings or codes assigned to instances of E1 CRM Entity in order to identify them uniquely and permanently within the context of one or more organisations. Such codes are often known as inventory numbers, registration codes, etc. and are typically composed of alphanumeric sequences. The class E42 Identifier is not normally used for machine-generated identifiers used for automated processing unless these are also used by human agents.

Examples:
- \"MM.GE.195\"
- \"13.45.1976\"
- \"OXCMS: 1997.4.1\"
- ISSN \"0041-5278\"
- ISRC \"FIFIN8900116\"
- Shelf mark \"Res 8 P 10\"
- \"Guillaume de Machaut (1300?-1377)\" [a controlled personal name heading that follows
the French rules]

In First Order Logic:
E42(x) ⊃ E41(x)"@en .



cidoc:E44_Place_Appellation
rdfs:comment "Scope note:
This class comprises any sort of identifier characteristically used to refer to an E53 Place.

Instances of E44 Place Appellation may vary in their degree of precision and their meaning may vary over time - the same instance of E44 Place Appellation may be used to refer to several places, either because of cultural shifts, or because objects used as reference points have moved around. Instances of E44 Place Appellation can be extremely varied in form: postal addresses, instances of E47 Spatial Coordinate, and parts of buildings can all be considered as instances of E44 Place Appellation.

Examples:
- \"Vienna\"
- \"CH-1211, Genève\"
- \"Aquae Sulis Minerva\"
- \"Bath\"
- \"Cambridge\"
- \"the Other Place\"
- \"the City\"

In First Order Logic:
E44(x) ⊃ E41(x)"@en .

cidoc:E45_Address
rdfs:comment "Scope note:
This class comprises identifiers expressed in coding systems for places, such as postal addresses used for mailing.

An E45 Address can be considered both as the name of an E53 Place and as an E51 Contact Point for an E39 Actor. This dual aspect is reflected in the multiple inheritance. However, some forms of mailing addresses, such as a postal box, are only instances of E51 Contact Point, since they do not identify any particular Place. These should not be documented as instances of E45 Address.

Examples:
- \"1-29-3 Otsuka, Bunkyo-ku, Tokyo, 121, Japan\"
- \"Rue David Dufour 5, CH-1211, Genève\"

In First Order Logic:
E45(x) ⊃ E44(x)
E45(x) ⊃ E51(x)"@en .

cidoc:E46_Section_Definition
rdfs:comment "Scope note:
This class comprises areas of objects referred to in terms specific to the general geometry or structure of its kind.

The 'prow' of the boat, the 'frame' of the picture, the 'front' of the building are all instances of E46 Section Definition. The class highlights the fact that parts of objects can be treated as locations. This holds in particular for features without natural boundaries, such as the \"head\" of a marble statue made out of one block (cf. E53 Place). In answer to the question 'where is the signature?' one might reply 'on the lower left corner'. (Section Definition is closely related to the term \"segment\" in Gerstl, P.& Pribbenow, S, 1996 \" A conceptual theory of part – whole relations and its applications\", Data & Knowledge Engineering 20 305-322, North Holland- Elsevier).

Examples:
- \"the entrance lobby to the Ripley Center\"
- \"the poop deck of H.M.S Victory\"
- \"the Venus de Milo's left buttock\"
- \"left inner side of my box\"

In First Order Logic:
E46(x) ⊃ E44(x)"@en .

cidoc:E47_Spatial_Coordinates
rdfs:comment "Scope note:
This class comprises the textual or numeric information required to locate specific instances of E53 Place within schemes of spatial identification.

Coordinates are a specific form of E44 Place Appellation, that is, a means of referring to a particular E53 Place. Coordinates are not restricted to longitude, latitude and altitude. Any regular system of reference that maps onto an E19 Physical Object can be used to generate coordinates.

Examples:
- \"6°5'29\"N 45°12'13\"W\"
- \"Black queen's bishop 4\" [chess coordinate].

In First Order Logic:
E47(x) ⊃ E44(x)"@en .

cidoc:E48_Place_Name
rdfs:comment "Scope note:
This class comprises particular and common forms of E44 Place Appellation.

Place Names may change their application over time: the name of an E53 Place may change, and a name may be reused for a different E53 Place. Instances of E48 Place Name are typically subject to place name gazetteers.

Examples:
- \"Greece\"
- \"Athens\"
- \"Geneva\"
- \"Lac Léman\"

In First Order Logic:
E48(x) ⊃ E44(x)"@en .

cidoc:E49_Time_Appellation
rdfs:comment "Scope note:
This class comprises all forms of names or codes, such as historical periods, and dates, which are characteristically used to refer to a specific E52 Time-Span.

The instances of E49 Time Appellation may vary in their degree of precision, and they may be relative to other time frames, \"Before Christ\" for example. Instances of E52 Time-Span are often defined by reference to a cultural period or an event e.g. 'the duration of the Ming Dynasty'.

Examples:
- \"Meiji\" [Japanese term for a specific time-span]
- \"1st half of the XX century\"
- \"Quaternary\"
- \"1215 Hegira\" [a date in the Islamic calendar]
- \"Last century\"

In First Order Logic:
E49(x) ⊃ E41(x)"@en .


cidoc:E50_Date
rdfs:comment "Scope note:
This class comprises specific forms of E49 Time Appellation.

Dates may vary in their degree of precision.

Examples:
- \"1900\"
- \"4-4-1959\"
- \"19-MAR-1922\"
- \"19640604\"

In First Order Logic:
E50(x) ⊃ E49(x)"@en .

cidoc:E51_Contact_Point
rdfs:comment "Scope note:
This class comprises identifiers employed, or understood, by communication services to direct communications to an instance of E39 Actor. These include E-mail addresses, telephone numbers, post office boxes, Fax numbers, URLs etc. Most postal addresses can be considered both as instances of E44 Place Appellation and E51 Contact Point. In such cases the subclass E45 Address should be used.
URLs are addresses used by machines to access another machine through an http request. Since the accessed machine acts on behalf of the E39 Actor providing the machine, URLs are considered as instances of E51 Contact Point to that E39 Actor.

Examples:
- \"+41 22 418 5571\"
- \"weasel@paveprime.com\"

In First Order Logic:
E51(x) ⊃ E41(x)"@en .

cidoc:E52_Time-Span
rdfs:comment "Scope note:
This class comprises abstract temporal extents, in the sense of Galilean physics, having a beginning, an end and a duration.

Time Span has no other semantic connotations. Time-Spans are used to define the temporal extent of instances of E4 Period, E5 Event and any other phenomena valid for a certain time. An E52 Time-Span may be identified by one or more instances of E49 Time Appellation.

Since our knowledge of history is imperfect, instances of E52 Time-Span can best be considered as approximations of the actual Time-Spans of temporal entities. The properties of E52 Time-Span are intended to allow these approximations to be expressed precisely.  An extreme case of approximation, might, for example, define an E52 Time-Span having unknown beginning, end and duration. Used as a common E52 Time-Span for two events, it would nevertheless define them as being simultaneous, even if nothing else was known.

Automatic processing and querying of instances of E52 Time-Span is facilitated if data can be parsed into an E61 Time Primitive.

Examples:
- 1961
- from 12-17-1993 to 12-8-1996
- 14h30 - 16h22 4th July 1945
- 9.30 am 1.1.1999 to 2.00 pm 1.1.1999
- duration of the Ming Dynasty

In First Order Logic:
E52(x) ⊃ E1(x)"@en .

cidoc:E53_Place
rdfs:comment "Scope note:
This class comprises extents in space, in particular on the surface of the earth, in the pure sense of physics: independent from temporal phenomena and matter.

The instances of E53 Place are usually determined by reference to the position of \"immobile\" objects such as buildings, cities, mountains, rivers, or dedicated geodetic marks. A Place can be determined by combining a frame of reference and a location with respect to this frame. It may be identified by one or more instances of E44 Place Appellation.

It is sometimes argued that instances of E53 Place are best identified by global coordinates or absolute reference systems. However, relative references are often more relevant in the context of cultural documentation and tend to be more precise. In particular, we are often interested in position in relation to large, mobile objects, such as ships. For example, the Place at which Nelson died is known with reference to a large mobile object – H.M.S Victory. A resolution of this Place in terms of absolute coordinates would require knowledge of the movements of the vessel and the precise time of death, either of which may be revised, and the result would lack historical and cultural relevance.

Any object can serve as a frame of reference for E53 Place determination. The model foresees the notion of a \"section\" of an E19 Physical Object as a valid E53 Place determination.

Examples:
- the extent of the UK in the year 2003
- the position of the hallmark on the inside of my wedding ring
- the place referred to in the phrase: \"Fish collected at three miles north of the confluence of the Arve and the Rhone\"
- here -> <-

In First Order Logic:
E53(x) ⊃ E1(x)"@en .

cidoc:E54_Dimension
rdfs:comment "Scope note:
This class comprises quantifiable properties that can be measured by some calibrated means and can be approximated by values, i.e. points or regions in a mathematical or conceptual space, such as natural or real numbers, RGB values etc.

An instance of E54 Dimension represents the true quantity, independent from its numerical approximation, e.g. in inches or in cm. The properties of the class E54 Dimension allow for expressing the numerical approximation of the values of an instance of E54 Dimension. If the true values belong to a non-discrete space, such as spatial distances, it is recommended to record them as approximations by intervals or regions of indeterminacy enclosing the assumed true values. For instance, a length of 5 cm may be recorded as 4.5-5.5 cm, according to the precision of the respective observation. Note, that interoperability of values described in different units depends critically on the representation as value regions.

Numerical approximations in archaic instances of E58 Measurement Unit used in historical records should be preserved. Equivalents corresponding to current knowledge should be recorded as additional instances of E54 Dimension as appropriate.

Examples:
- currency: £26.00
- length: 3.9-4.1 cm
- diameter: 26 mm
- weight: 150 lbs
- density: 0.85 gm/cc
- luminescence: 56 ISO lumens
- tin content: 0.46 %
- taille au garot: 5 hands
- calibrated C14 date: 2460-2720 years, etc

In First Order Logic:
E54(x) ⊃ E1(x)"@en .

cidoc:E55_Type
rdfs:comment "Scope note:
This class comprises concepts denoted by terms from thesauri and controlled vocabularies used to characterize and classify instances of CRM classes. Instances of E55 Type represent concepts  in contrast to instances of E41 Appellation which are used to name instances of CRM classes.

E55 Type is the CRM's interface to domain specific ontologies and thesauri. These can be represented in the CRM as subclasses of E55 Type, forming hierarchies of terms, i.e. instances of E55 Type linked via P127 has broader  term (has narrower term). Such hierarchies may be extended with additional properties.

Examples:
- weight, length, depth [types of E54]
- portrait, sketch, animation [types of E38]
- French, English, German [E56]
- excellent, good, poor [types of E3]
- Ford Model T, chop stick [types of E22]
- cave, doline, scratch [types of E26]
- poem, short story [types of E33]
- wedding, earthquake, skirmish [types of E5]

In First Order Logic:
E55(x) ⊃ E28(x)"@en .

cidoc:E57_Material
rdfs:comment "Scope note:
This class is a specialization of E55 Type and comprises the concepts of materials.

Instances of E57 Material may denote properties of matter before its use, during its use, and as incorporated in an object, such as ultramarine powder, tempera paste, reinforced concrete. Discrete pieces of raw-materials kept in museums, such as bricks, sheets of fabric, pieces of metal, should be modelled individually in the same way as other objects. Discrete used or processed pieces, such as the stones from Nefer Titi's temple, should be modelled as parts (cf. P46 is composed of).

This type is used categorically in the model without reference to instances of it, i.e. the Model does not foresee the description of instances of instances of E57 Material, e.g.: \"instances of  gold\".

It is recommended that internationally or nationally agreed codes and terminology are used.

Examples:
- brick
- gold
- aluminium
- polycarbonate
- resin

In First Order Logic:
E57(x) ⊃ E55(x)"@en .

cidoc:E58_Measurement_Unit
rdfs:comment "Scope note:
This class is a specialization of E55 Type and comprises the types of measurement units: feet, inches, centimetres, litres, lumens, etc.

This type is used categorically in the model without reference to instances of it, i.e. the Model does not foresee the description of instances of instances of E58 Measurement Unit, e.g.: \"instances of cm\".

Système International (SI) units or internationally recognized non-SI terms should be used whenever possible. (ISO 1000:1992). Archaic Measurement Units used in historical records should be preserved.

Examples:
- cm [centrimetre]
- km [kilometre]
- m [meter]
- m/s [meters per second]
- A [Ampere]
- GRD [Greek Drachme]
- C° [degrees centigrade]

In First Order Logic:
E58(x) ⊃ E55(x)"@en .



cidoc:E70_Thing
rdfs:comment "Scope note:
This general class comprises discrete, identifiable, instances of E77 Persistent Item that are documented as single units, that either consist of matter or depend on being carried by matter and are characterized by relative stability. 

They may be intellectual products or physical things. They may for instance have a solid physical form, an electronic encoding, or they may be a logical concept or structure.

Examples:
- my photograph collection (E78)
- the bottle of milk in my refrigerator (E22)
- the plan of the Strassburger Muenster (E29)
- the thing on the top of Otto Hahn's desk (E19)
- the form of the no-smoking sign (E36)
- the cave of Dirou, Mani, Greece (E27)

In First Order Logic:
E70(x) ⊃ E77(x)"@en .

cidoc:E71_Man-Made_Thing
rdfs:comment "Scope note:
This class comprises discrete, identifiable man-made items that are documented as single units.

These items are either intellectual products or man-made physical things, and are characterized by relative stability. They may for instance have a solid physical form, an electronic encoding, or they may be logical concepts or structures.

Examples:
- Beethoven's 5th Symphony (E73)
- Michelangelo's David
- Einstein's Theory of General Relativity (E73)
- the taxon 'Fringilla coelebs Linnaeus, 1758' (E55)

In First Order Logic:
E71(x) ⊃ E70(x)"@en .

cidoc:E72_Legal_Object
rdfs:comment "Scope note:
This class comprises those material or immaterial items to which instances of E30 Right, such as the right of ownership or use, can be applied.

This is true for all E18 Physical Thing. In the case of instances of E28 Conceptual Object, however, the identity of the E28 Conceptual Object or the method of its use may be too ambiguous to reliably establish instances of E30 Right, as in the case of taxa and inspirations. Ownership of corporations is currently regarded as out of scope of the CRM.

Examples:
- the Cullinan diamond (E19)
- definition of the CIDOC Conceptual Reference Model Version 2.1 (E73)

In First Order Logic:
E72(x) ⊃ E70(x)"@en .

cidoc:E73_Information_Object
rdfs:comment "Scope note:
This class comprises identifiable immaterial items, such as a poems, jokes, data sets, images, texts, multimedia objects, procedural prescriptions, computer program code, algorithm or mathematical formulae, that have an objectively recognizable structure and are documented as single units.
The encoding structure known as a \"named graph\" also falls under this class, so that each \"named graph\" is an instance of an E73 Information Object.

An E73 Information Object does not depend on a specific physical carrier, which can include human memory, and it can exist on one or more carriers simultaneously.
Instances of E73 Information Object of a linguistic nature should be declared as instances of the E33 Linguistic Object subclass. Instances of E73 Information Object of a documentary nature should be declared as instances of the E31 Document subclass. Conceptual items such as types and classes are not instances of E73 Information Object, nor are ideas without a reproducible expression.

Examples:
- image BM000038850.JPG from the Clayton Herbarium in London
- E. A. Poe's \"The Raven\"
- the movie \"The Seven Samurai\" by Akira Kurosawa
- the Maxwell Equations
- The Getty AAT as published as Linked Open Data, accessed 1/10/2014

In First Order Logic: 
E73(x) ⊃ E89(x)  
E73(x) ⊃ E90(x)"@en .

cidoc:E74_Group
rdfs:comment "Scope note:
This class comprises any gatherings or organizations of E39 Actors that act collectively or in a similar way due to any form of unifying relationship. In the wider sense this class also comprises official positions which used to be regarded in certain contexts as one actor, independent of the current holder
of the office, such as the president of a country. In such cases, it may happen that the Group never had more than one member. A joint pseudonym (i.e., a name that seems indicative of an individual but that is actually used as a persona by two or more people) is a particular case of E74 Group.

A gathering of people becomes an E74 Group when it exhibits organizational characteristics usually typified by a set of ideas or beliefs held in common, or actions performed together. These might be communication, creating some common artifact, a common purpose such as study, worship, business, sports, etc. Nationality can be modelled as membership in an E74 Group (cf. HumanML markup). Married couples and other concepts of family are regarded as particular examples of E74 Group. 

Examples:
- the impressionists
- the Navajo
- the Greeks
- the peace protestors in New York City on February 15 2003
- Exxon-Mobil
- King Solomon and his wives
- the President of the Swiss Confederation
- Nicolas Bourbaki 
- Betty Crocker
- Ellery Queen

In First Order Logic:
E74(x) ⊃ E39(x)"@en .

cidoc:E75_Conceptual_Object_Appellation
rdfs:comment "Scope note:
This class comprises all appellations specific to intellectual products or standardized patterns.
This class comprises appellations that are by their form or syntax specific to identifying instances of
E28 Conceptual Object, such as intellectual products, standardized patterns etc.


Examples:
- \"ISBN 3-7913-1418-1\"
- \"ISO 2788-1986 (F)\"
- \"DOI=10.1109/MIS.2007.103\"

In First Order Logic:
E75(x) ⊃ E41(x)"@en .

cidoc:E77_Persistent_Item
rdfs:comment "Scope note:
This class comprises items that have a persistent identity, sometimes known as \"endurants\" in philosophy.

They can be repeatedly recognized within the duration of their existence by identity criteria rather than by continuity or observation. Persistent Items can be either physical entities, such as people, animals or things, or conceptual entities such as ideas, concepts, products of the imagination or common names. 

The criteria that determine the identity of an item are often difficult to establish -; the decision depends largely on the judgement of the observer. For example, a building is regarded as no longer existing if it is dismantled and the materials reused in a different configuration. On the other hand, human beings go through radical and profound changes during their life-span, affecting both material composition and form, yet preserve their identity by other criteria. Similarly, inanimate objects may be subject to exchange of parts and matter. The class E77 Persistent Item does not take any position about the nature of the applicable identity criteria and if actual knowledge about identity of an instance of this class exists. There may be cases, where the identity of an E77 Persistent Item is not decidable by a certain state of knowledge.
The main classes of objects that fall outside the scope the E77 Persistent Item class are temporal objects such as periods, events and acts, and descriptive properties.

Examples:
- Leonardo da Vinci
- Stonehenge
- the hole in the ozone layer
- the First Law of Thermodynamics
- the Bermuda Triangle

In First Order Logic:
E77(x) ⊃ E1(x)"@en .

cidoc:E79_Part_Addition 
rdfs:comment "
This class comprises activities that result in an instance of E24 Physical Man-Made Thing being increased, enlarged or augmented by the addition of a part. 
 
Typical scenarios include the attachment of an accessory, the integration of a component, the addition of an element to an aggregate object, or the accessioning of an object into a curated E78 Collection. Objects to which parts are added are, by definition, man-made, since the addition of a part implies a human activity. Following the addition of parts, the resulting man-made assemblages are treated objectively as single identifiable wholes, made up of constituent or component parts bound together either physically (for example the engine becoming a part of the car), or by sharing a common purpose (such as the 32 chess pieces that make up a chess set). This class of activities forms a basis for reasoning about the history and continuity of identity of objects that are integrated into other objects over time, such as precious gemstones being repeatedly incorporated into different items of jewellery, or cultural artifacts being added to different museum instances of E78 Collection over their lifespan.
 
Examples:

    the setting of the koh-i-noor diamond into the crown of Queen Elizabeth the Queen Mother
    the addition of the painting 'Room in Brooklyn' by Edward Hopper to the collection of the Museum of Fine Arts, Boston

 
In First Order Logic:
E79(x) ⊃ E11(x)
Outgoing Direct Properties:
E79 Part Addition. P110 augmented (was augmented by) : E24 Physical Man-Made Thing,
E79 Part Addition. P111 added (was added by) : E18 Physical Thing
"@en .
            

cidoc:E80_Part_Removal 
rdfs:comment "This class comprises the activities that result in an instance of E18 Physical Thing being decreased by the removal of a part.
 
Typical scenarios include the detachment of an accessory, the removal of a component or part of a composite object, or the deaccessioning of an object from a curated E78 Collection. If the E80 Part Removal results in the total decomposition of the original object into pieces, such that the whole ceases to exist, the activity should instead be modelled as an E81 Transformation, i.e. a simultaneous destruction and production. In cases where the part removed has no discernible identity prior to its removal but does have an identity subsequent to its removal, the activity should be regarded as both E80 Part Removal and E12 Production. This class of activities forms a basis for reasoning about the history, and continuity of identity over time, of objects that are removed from other objects, such as precious gemstones being extracted from different items of jewelry, or cultural artifacts being deaccessioned from different museum collections over their lifespan.
 
Examples:

    the removal of the engine from my car
    the disposal of object number 1976:234 from the collection

 
In First Order Logic:
E80(x) ⊃ E11(x)
Outgoing Direct Properties:
E80 Part Removal. P112 diminished (was diminished by) : E24 Physical Man-Made Thing,
E80 Part Removal. P113 removed (was removed by) : E18 Physical Thing
"@en. 


cidoc:E82_Actor_Appellation
rdfs:comment "Scope note:
This class comprises any sort of name, number, code or symbol characteristically used to identify an E39 Actor.
An E39 Actor will typically have more than one E82 Actor Appellation, and instances of E82 Actor Appellation in turn may have alternative representations. The distinction between corporate and personal names, which is particularly important in library applications, should be made by explicitly linking the E82 Actor Appellation to an instance of either E21 Person or E74 Group/E40 Legal Body. If this is not possible, the distinction can be made through the use of the P2 has type mechanism.

Examples:
- \"John Doe\"
- \"Doe, J\"
- \"the U.S. Social Security Number 246-14-2304\"
- \"the Artist Formerly Known as Prince\"
- \"the Master of the Flemish Madonna\"
- \"Raphael's Workshop\"
- \"the Brontë Sisters\"
- \"ICOM\"
- \"International Council of Museums\"

In First Order Logic:
E82(x) ⊃ E41(x)"@en .

cidoc:E89_Propositional_Object
rdfs:comment "Scope note:
This class comprises immaterial items, including but not limited to stories, plots, procedural prescriptions, algorithms, laws of physics or images that are, or represent in some sense, sets of propositions about real or imaginary things and that are documented as single units or serve as topic of discourse.

This class also comprises items that are \"about\" something in the sense of a subject. In the wider sense, this class includes expressions of psychological value such as non-figural art and musical themes. However, conceptual items such as types and classes are not instances of E89 Propositional Object. This should not be confused with the definition of a type, which is indeed an instance of E89 Propositional Object.

Examples:
- Maxwell's Equations
- The ideational contents of Aristotle's book entitled 'Metaphysics' as rendered in the Greek texts translated in … Oxford edition…
- The underlying prototype of any \"no-smoking\" sign (E36)
- The common ideas of the plots of the movie \"The Seven Samurai\" by Akira Kurosawa and the movie \"The Magnificent Seven\" by John Sturges
- The image content of the photo of the Allied Leaders at Yalta published by UPI, 1945 (E38)

In First Order Logic:
E89(x) ⊃ E28(x)"@en .


cidoc:E90_Symbolic_Object
rdfs:comment "Scope note:
This class comprises identifiable symbols and any aggregation of symbols, such as characters, identifiers, traffic signs, emblems, texts, data sets, images, musical scores, multimedia objects, computer program code or mathematical formulae that have an objectively recognizable structure and that are documented as single units. 

It includes sets of signs of any nature, which may serve to designate something, or to communicate some propositional content.

An instance of E90 Symbolic Object does not depend on a specific physical carrier, which can include human memory, and it can exist on one or more carriers simultaneously. An instance of E90 Symbolic Object may or may not have a specific meaning, for example an arbitrary character string. 

In some cases, the content of an instance of E90 Symbolic Object may completely be represented by a serialized digital content model, such as a sequence of ASCII-encoded characters, an XML or HTML document, or a TIFF image. The property P3 has note allows for the description of this content model. In order to disambiguate which symbolic level is the carrier of the meaning, the property P3.1 has type can be used to specify the encoding (e.g. \"bit\", \"Latin character\", RGB pixel). 

Examples:
- 'ecognizabl' 
- The \"no-smoking\" sign (E36) 
- \"BM000038850.JPG\" (E75) 
- image BM000038850.JPG from the Clayton Herbarium in London (E38) 
- The distribution of form, tone and colour found on Leonardo da Vinci's painting named \"Mona Lisa\" in daylight (E38)
- The Italian text of Dante's \"Divina Commedia\" as found in the authoritative critical edition La Commedia secondo l'antica vulgata a cura di Giorgio Petrocchi, Milano: Mondadori, 1966-67 (= Le Opere di Dante Alighieri, Edizione Nazionale a cura della Società Dantesca Italiana, VII, 1-4) (E33)

In First Order Logic:
E90(x) ⊃ E28(x)
E90(x) ⊃ E72(x)"@en .



cidoc:P1_is_identified_by rdfs:label "P1 is identified by"@en.
cidoc:P1i_identifies rdfs:label "P1i identifies"@en.
cidoc:P2_has_type rdfs:label "P2 has type"@en.
cidoc:P2i_is_type_of rdfs:label "P2i is type of"@en.
cidoc:P3_has_note rdfs:label "P3 has note"@en.
cidoc:P4_has_time-span rdfs:label "P4 has time-span"@en.
cidoc:P4i_is_time-span_of rdfs:label "P4i is time-span of"@en.
cidoc:P5_consists_of rdfs:label "P5 consists of"@en.
cidoc:P5i_forms_part_of rdfs:label "P5i forms part of"@en.
cidoc:P8_took_place_on_or_within rdfs:label "P8 took place on or within"@en.
cidoc:P8i_witnessed rdfs:label "P8i witnessed"@en.
cidoc:P14_carried_out_by rdfs:label "P14 carried out by"@en.
cidoc:P14i_performed rdfs:label "P14i performed"@en.

cidoc:P43_has_dimension rdfs:label "P43 has dimension"@en.
cidoc:P43i_is_dimension_of rdfs:label "P43i is dimension of"@en.
cidoc:P45_consists_of rdfs:label "P45 consists of"@en.
cidoc:P45i_is_incorporated_in rdfs:label "P45i is incorporated in"@en.
cidoc:P46_is_composed_of rdfs:label "P46 is composed of"@en.
cidoc:P46i_forms_part_of rdfs:label "P46i forms part of"@en.
cidoc:P54_has_current_permanent_location rdfs:label "P54 has current permanent location"@en.
cidoc:P54i_is_current_permanent_location_of rdfs:label "P54i is current permanent location of"@en.
cidoc:P56_bears_feature rdfs:label "P56 bears feature"@en.
cidoc:P56i_is_found_on rdfs:label "P56i is found on"@en.
cidoc:P67_refers_to rdfs:label "P67 refers to"@en.
cidoc:P67i_is_referred_by rdfs:label "P67i is referred by"@en.
cidoc:P68_foresees_use_of rdfs:label "P68 foresees use of"@en.
cidoc:P68i_use_foreseen_by rdfs:label "P68i use foreseen by"@en.
cidoc:P81_ongoing_throughout rdfs:label "P81 ongoing throughout"@en.
cidoc:P82_at_some_time_within rdfs:label "P82 at some time within"@en.
cidoc:P83_had_at_least_duration rdfs:label "P83 had at least duration"@en.
cidoc:P83i_was_minimum_duration_of rdfs:label "P83i was minimum duration of"@en.
cidoc:P84_had_at_most_duration rdfs:label "P84 had at most duration"@en.
cidoc:P84i_was_maximum_duration_of rdfs:label "P84i was maximum duration of"@en.
cidoc:P90_has_value rdfs:label "P90 has value"@en.
cidoc:P91_has_unit rdfs:label "P91 has unit"@en.
cidoc:P91i_is_unit_of rdfs:label "P91i is unit of"@en .
cidoc:P115_finishes  rdfs:label "P115 finishes"@en.
cidoc:P115i_is_finished_by rdfs:label "P115i is finished by"@en.
cidoc:P116_starts rdfs:label "P116 starts"@en.
cidoc:P116i_is_started_by rdfs:label "P116i is started by"@en.
cidoc:P127_has_broader_term rdfs:label "P127 has broader term"@en.
cidoc:P127i_has_narrower_term rdfs:label "P127i has narrower term"@en.
cidoc:P140_assigned_attribute_to rdfs:label "P140 assigned attribute to"@en.
cidoc:P140i_was_attributed_by rdfs:label "P140i was attributed by"@en.
cidoc:P141_assigned rdfs:label "P141 assigned"@en.
cidoc:P141i_was_assigned_by rdfs:label "P141i was assigned by"@en.
cidoc:P148_has_component rdfs:label "P148 has component"@en.
cidoc:P148i_is_component_of rdfs:label "P148i is component of"@en.

BldgCitygml2:lod0FootPrint rdfs:label "PG1 lod0FootPrint"@en.
bcho:PG1i_lod0FootPrint_of rdfs:label "PG1i lod0FootPrint of"@en.
BldgCitygml2:lod0RoofEdge rdfs:label "PG2 lod0RoofEdge"@en.
bcho:PG2i_lod0RoofEdge_of rdfs:label "PG2i lod0RoofEdge of"@en.
BldgCitygml2:lod1Solid rdfs:label "PG3 lod1Solid"@en.
bcho:PG3i_lod1Solid_of rdfs:label "PG3i lod1Solid of"@en.
BldgCitygml2:outerBuildingInstallation rdfs:label "PG4 outerBuildingInstallation"@en.
bcho:PG4i_outerBuildingInstallation_of rdfs:label "PG4i outerBuildingInstallation of"@en.
bcho:PG5i_bounded rdfs:label "PG5i bounded"@en.
BldgCitygml2:boundedBy rdfs:label "PG5 bounded by"@en.
BldgCitygml2:lod2MultiSurface rdfs:label "PG6 lod2MultiSurface"@en.
bcho:PG6i_lod2MultiSurface_of rdfs:label "PG6i lod2MultiSurface of"@en.
BldgCitygml2:lod3MultiSurface rdfs:label "PG7 lod3MultiSurface"@en.
bcho:PG7i_lod3MultiSurface_of rdfs:label "PG7i lod3MultiSurface of"@en.
BldgCitygml2:opening rdfs:label "PG8 opening"@en.
bcho:PG8i_opening_of rdfs:label "PG8i opening of"@en.
BldgCitygml2:lod4Solid rdfs:label "PG9 lod4Solid"@en.
bcho:PG9i_lod4Solid_of rdfs:label "PG9i lod4Solid of"@en.
BldgCitygml2:lod4MultiSurface rdfs:label "PG10 lod4MultiSurface"@en.
bcho:PG10i_lod4MultiSurface_of rdfs:label "PG10i lod4MultiSurface of"@en.
bcho:PG11_lod4Geometry rdfs:label "PG11 lod4Geometry"@en.
bcho:PG11i_lod4Geometry_of rdfs:label "PG11i lod4Geometry of"@en.

bcho:PHB1_has_scope rdfs:label "PHB1 has scope"@en.
bcho:PHB1i_is_scope_of rdfs:label "PHB1i is scope of"@en.
bcho:PHB2_has_courtyard rdfs:label "PHB2 has courtyard"@en.
bcho:PHB3_has_orchard rdfs:label "PHB3 has orchard"@en.
bcho:PHB4_has_agent rdfs:label "PHB4 has agent"@en.
bcho:PHB4i_is_agent_of rdfs:label "PHB4i is agent of"@en.
bcho:PHB5_has_damage rdfs:label "PHB5 has damage"@en.
bcho:PHB5i_is_damage_of rdfs:label "PHB5i is damage of"@en.
bcho:PHB6_has_weight rdfs:label "PHB6 has weight"@en.
bcho:PHB7_has_vulnerability_parameter rdfs:label "PHB7 has vulnerability parameter"@en.
bcho:PHB7i_is_damage_vulnerability_parameter_of rdfs:label "PHB7i is damage vulnerability parameter of"@en.
bcho:PHB8_has_condition_value rdfs:label "PHB8 has condition value"@en.
bcho:PHB9_has_condition_weight rdfs:label "PHB9 has condition weight"@en.
bcho:PHB10_has_condition_variable rdfs:label "PHB10 has condition variable"@en.
bcho:PHB10i_is_condition_variable_of rdfs:label "PHB10i is condition variable of"@en.
bcho:PHB11_has_condition rdfs:label "PHB11 has condition"@en.
bcho:PHB11i_refers_to_value rdfs:label "PHB11i refers to value"@en.
bcho:PHB12_has_parameter rdfs:label "PHB12 has parameter"@en.
bcho:PHB12i_is_parameter_of rdfs:label "PHB12i is parameter of"@en.
bcho:PHB13_has_max_limit rdfs:label "PHB13 has max limit"@en.
bcho:PHB14_has_min_limit rdfs:label "PHB14 has min limit"@en.
bcho:PHB15_has_therapy rdfs:label "PHB15 has therapy"@en.
bcho:PHB15i_is_therapy_of rdfs:label "PHB15i is therapy of"@en.
bcho:PHB16_has_suggested_action rdfs:label "PHB16 has suggested action"@en.
bcho:PHB16i_is_suggested_action_of rdfs:label "PHB16i is suggested action of"@en.
bcho:PHB17_has_status rdfs:label "PHB17 has status"@en.
bcho:PHB17i_is_status_of rdfs:label "PHB17i is status of"@en.
bcho:PHB18_has_budget rdfs:label "PHB18 has budget"@en.
bcho:PHB19_has_resource rdfs:label "PHB19 has resource"@en.
bcho:PHB19i_is_resource_of rdfs:label "PHB19i is resource of"@en.
bcho:PHB20_has_intervention rdfs:label "PHB20 has intervention"@en.
bcho:PHB20i_is_intervention_of rdfs:label "PHB20i is intervention of"@en.
bcho:PHB21_has_intervention_action rdfs:label "PHB21 has intervention action"@en.
bcho:PHB21i_is_intervention_action_of rdfs:label "PHB21i is intervention action of"@en.
bcho:PHB22_requires_further_inspections rdfs:label "PHB22 requires further inspections"@en.
bcho:PHB23_conservation_objective_reached rdfs:label "PHB23 conservation objective reached"@en.
bcho:PHB24_has_inspection rdfs:label "PHB24 has inspection"@en.
bcho:PHB24i_is_inspection_of rdfs:label "PHB24i is inspection of"@en.
bcho:PHB25_has_geographical_representation rdfs:label "PHB25 has geographical representation"@en.
bcho:PHB25i_is_representation_of rdfs:label "PHB25i is representation of"@en.


bcho:PM1i_is_subject_to_risk rdfs:label "PM1i is subject to risk"@en.
mondis:refersToHazard rdfs:label "PM1 refers to hazard"@en.
mondis:isSubjectedTo rdfs:label "PM2 is subject to"@en.
bcho:PM2i_refers_to rdfs:label "PM2i refers to"@en.
bcho:PM3i_eliminates rdfs:label "PM3i eliminates"@en.
mondis:isEliminatedByIntervention rdfs:label "PM3 is eliminated by intervention"@en.
mondis:isRepairOfDamage rdfs:label "PM4 is repair of damage"@en.
bcho:PM4i_is_repaired_on rdfs:label "PM4i is repaired on"@en.




bcho:PHB1_has_scope
rdfs:comment "The 'PHB1 has scope' property links the 'E40 Legal body' class with the scope."@en.
bcho:PHB1i_is_scope_of rdfs:comment "Inverse property of 'bcho:PHB1_has_scope'."@en.

bcho:PHB2_has_courtyard
rdfs:comment "'PHB2 has courtyard' and 'PHB3 has orchard' properties link the 'HB32 Organizational Aspect' class with its value."@en.

bcho:PHB3_has_orchard
rdfs:comment "'PHB2 has courtyard' and 'PHB3 has orchard' properties link the 'HB32 Organizational Aspect' class with its value."@en.

bcho:PHB4_has_agent
rdfs:comment "The property 'PHB4 has agent' relates damages to deterioration agents."@en.
bcho:PHB4i_is_agent_of rdfs:comment "Inverse property of 'bcho:PHB4_has_agent'."@en.

bcho:PHB5_has_damage
rdfs:comment "The 'PHB5 has damage' property relates gravity to damages."@en.
bcho:PHB5i_is_damage_of rdfs:comment "Inverse property of 'bcho:PHB5_has_damage'."@en.

bcho:PHB6_has_weight
rdfs:comment "To compute the vulnerability a new class 'HB42 Vulnerability Parameter' was created. These parameters are accompanied by a weight, since not all the parameters have the same importance; therefore the 'HBP6 has weight' property has also been added."@en.

bcho:PHB7_has_vulnerability_parameter
rdfs:comment "The 'PHB7 has vulnerability parameter' property relates parameters to vulnerability."@en.
bcho:PHB7i_is_damage_vulnerability_parameter_of rdfs:comment "Inverse property of 'bcho:PHB7_has_vulnerability_parameter'."@en.

bcho:PHB8_has_condition_value
rdfs:comment "The 'HB44 Condition Variable Assignment' class was created under the 'E14 Condition Assessment' class and it links condition variables with their value and the weight through the 'PHB8 has condition value' and 'PHB9 has condition weight' properties."@en.

bcho:PHB9_has_condition_weight
rdfs:comment "The 'HB44 Condition Variable Assignment' class was created under the 'E14 Condition Assessment' class and it links condition variables with their value and the weight through the 'PHB8 has condition value' and 'PHB9 has condition weight' properties."@en.

bcho:PHB10_has_condition_variable
rdfs:comment "The 'PHB10 has condition variable' property links the condition variable to the assignment."@en.
bcho:PHB10i_is_condition_variable_of rdfs:comment "Inverse property of 'bcho:PHB10_has_condition_variable'."@en.

bcho:PHB11_has_condition rdfs:comment "General condition is linked to the heritage value with the 'PHB11 refers to value' property."@en.
bcho:PHB11i_refers_to_value rdfs:comment "Inverse property of 'bcho:PHB11_refers_to_value'."@en.

bcho:PHB12_has_parameter
rdfs:comment "The 'PHB12 has parameter' property links the performance status with its parameters."@en.
bcho:PHB12i_is_parameter_of rdfs:comment "Inverse property of 'bcho:PHB12_has_parameter'."@en.

bcho:PHB13_has_max_limit
rdfs:comment "'PHB13 has max limit' and 'PHB14 has min limit' properties establish thresholds for the performance status parameters."@en.

bcho:PHB14_has_min_limit
rdfs:comment "'PHB13 has max limit' and 'PHB14 has min limit' properties establish thresholds for the performance status parameters."@en.

bcho:PHB15_has_therapy
rdfs:comment "The 'PHB15 has therapy' property links the suggested therapy with the performance status."@en.
bcho:PHB15i_is_therapy_of rdfs:comment "Inverse property of 'bcho:PHB15_has_therapy'."@en.

bcho:PHB16_has_suggested_action
rdfs:comment "The 'PHB16 has suggested action' property links the therapy with the suggested actions."@en.  
bcho:PHB16i_is_suggested_action_of rdfs:comment "Inverse property of 'bcho:PHB16_has_suggested_action'."@en.

bcho:PHB17_has_status
rdfs:comment "The 'PHB17 has status' property links the action status to the suggested action."@en.
bcho:PHB17i_is_status_of rdfs:comment "Inverse property of 'bcho:PHB17_has_status'."@en.

bcho:PHB18_has_budget
rdfs:comment "The 'PHB18 has budget' and 'PHB19 has resource' properties associate a budget and the resources needed for the execution of the suggested action."@en.

bcho:PHB19_has_resource
rdfs:comment "The 'PHB18 has budget' and 'PHB19 has resource' properties associate a budget and the resources needed for the execution of the suggested action."@en.
bcho:PHB19i_is_resource_of rdfs:comment "Inverse property of 'bcho:PHB19_has_resource'."@en.

bcho:PHB20_has_intervention
rdfs:comment "During the therapy phase an intervention is executed. The MONDIS 'M28 Intervention' class is used to keep track of the suggested actions used in the intervention. The suggested therapy is linked to the intervention through the 'PHB20 has intervention' property."@en.
bcho:PHB20i_is_intervention_of rdfs:comment "Inverse property of 'bcho:PHB20_has_intervention'."@en.

bcho:PHB21_has_intervention_action
rdfs:comment "An individual action used during the intervention is recorded through the 'HB49 Action' class. The 'PHB21 has intervention action' property links the intervention with the action. The 'HB51 Action Status' class instantiated as 'executed action' means that the suggested therapy action was executed in the intervention."@en.
bcho:PHB21i_is_intervention_action_of rdfs:comment "Inverse property of 'bcho:PHB21_has_intervention_action'."@en.

bcho:PHB22_requires_further_inspections
rdfs:comment "The control phase ends with one or more inspections to verify whether the actions reached the conservation objective. The 'PHB22 requires further inspections' property means that more control activities are required."@en.

bcho:PHB23_conservation_objective_reached
rdfs:comment "The control phase ends with one or more inspections to verify whether the actions reached the conservation objective. The 'PHB22 requires further inspections' property means that more control activities are required. The 'PHB23 conservation objective reached' property points out whether the conservation objective has been reached."@en.

bcho:PHB24_has_inspection
rdfs:comment "The control phase ends with one or more inspections to verify whether the actions reached the conservation objective. The therapy is linked to the inspection through the 'PHB24 has inspection' property."@en.
bcho:PHB24i_is_inspection_of rdfs:comment "Inverse property of 'bcho:PHB24_has_inspection'."@en.

bcho:PHB25_has_geographical_representation
rdfs:comment "the 'PHB25 has geographical representation' property connects the 'E1 CRM Entity' with the 'G11 MultiSurface' class, thus also other elements from the ontology such as: hazards, damages, etc. can be represented."@en.
bcho:PHB25i_is_representation_of rdfs:comment "Inverse property of 'bcho:PHB25_has_geographical_representation'."@en.






BldgCitygml2:lod0FootPrint 
rdfs:comment "The 'GP1 lod0 footprint' and 'GP2 lod0 roof edge' properties are used to link the abstract building to the multisurface."@en.

bcho:PG1i_lod0FootPrint_of rdfs:comment "Inverse property of 'PG1 lod0FootPrint'."@en.

BldgCitygml2:lod0RoofEdge                      
rdfs:comment "The 'PG1 lod0 footprint' and 'PG2 lod0 roof edge' properties are used to link the abstract building to the multisurface."@en.

bcho:PG2i_lod0RoofEdge_of rdfs:comment "Inverse property of 'PG2 lod0RoofEdge'."@en.

BldgCitygml2:lod1Solid
rdfs:comment "The outer shell of the building is represented in the second level of detail LOD1 as a block by the 'G7 Solid' class. The 'PG3 lod1 solid' property links the solid with the building."@en.

bcho:PG3i_lod1Solid_of rdfs:comment "Inverse property of 'PG3 lod1Solid'."@en.

BldgCitygml2:outerBuildingInstallation
rdfs:comment "The 'PG4 outer building installation' property links the abstract building with the building installation.". 

bcho:PG4i_outerBuildingInstallation_of rdfs:comment "Inverse property of 'PG4 outer Building Installation'."@en.

BldgCitygml2:boundedBy
rdfs:comment "The 'GP5 bounded by' property described 'G32 Room' and 'G19 Building Installation' instances bounded by 'G20 Boundary Sourface'."@en.

bcho:PG5i_bounded rdfs:comment "Inverse property of 'PG5 bounded by'."@en.

BldgCitygml2:lod2MultiSurface         
rdfs:comment "Boundary surfaces are linked to multisurfaces through the 'PG6 lod2 multisurface' property."@en.

bcho:PG6i_lod2MultiSurface_of rdfs:comment "Inverse property of 'PG6 lod2 multisurface'."@en.

BldgCitygml2:lod3MultiSurface
rdfs:comment "Openings are represented in LOD3 by the 'G29 Opening' class and the 'G30 Door' and 'G31 Window' subclasses. The geometry is represented by multisurfaces through the property 'PG7 lod3 multisurface'."@en.

bcho:PG7i_lod3MultiSurface_of rdfs:comment "Inverse property of 'PG7 lod3 multisurface'."@en.

BldgCitygml2:opening
rdfs:comment "Openings are represented in LOD3 by the 'G29 Opening' class and the 'G30 Door' and 'G31 Window' subclasses.  An opening in a boundary surface is represented using the property 'GP8 opening'."@en.

bcho:PG8i_opening_of rdfs:comment "Inverse property of 'GP8 opening'."@en.

BldgCitygml2:lod4Solid
rdfs:comment "Room geometry is represented by solids or multisurfaces through the 'PG9 lod4Solid' and 'PG10 lod4 multisurface' properties.".

bcho:PG9i_lod4Solid_of rdfs:comment "Inverse property of 'PG9 lod4Solid'."@en.

BldgCitygml2:lod4MultiSurface
rdfs:comment "Room geometry is represented by solids or multisurfaces through the 'PG9 lod4Solid' and 'GP10 lod4 multisurface' properties." .                               
bcho:PG10i_lod4MultiSurface_of rdfs:comment "Inverse property of 'PG10 lod4MultiSurface'."@en.

bcho:PG11_lod4Geometry
rdfs:comment "Furniture and interior building installations are represented using any set of geometries through the 'GP12 lod4 geometry' property.".

bcho:PG11i_lod4Geometry_of rdfs:comment "Inverse property of 'PG11_lod4Geometry'."@en.




mondis:isEliminatedByIntervention
rdfs:comment "'PM3 is eliminated by intervention' 'PM4 is repair of damage' properties link the agent and damage that are tackled by the intervention.".
bcho:PM4i_is_repaired_on rdfs:comment "Inverse property of 'PM4 is repair of damage'."@en.

mondis:isRepairOfDamage
rdfs:comment "'PM3 is eliminated by intervention' 'PM4 is repair of damage' properties link the agent and damage that are tackled by the intervention.".
bcho:PM3i_eliminates rdfs:comment "Inverse property of 'PM3 is eliminated by intervention'."@en.

mondis:isSubjectedTo
rdfs:comment "'PM2 is subject to' property links vulnerability with hazard.".
bcho:PM2i_refers_to rdfs:comment "Inverse property of 'PM2 is subject to'."@en.

mondis:refersToHazard
rdfs:comment "'PM1 refers to hazard' property links hazard with risk.".
bcho:PM1i_is_subject_to_risk rdfs:comment "Inverse property of 'PM1 refers to hazard'."@en.



cidoc:P1_is_identified_by
rdfs:comment "Scope note:
This property describes the naming or identification of any real world item by a name or any other identifier.

This property is intended for identifiers in general use, which form part of the world the model intends to describe, and not merely for internal database identifiers which are specific to a technical system, unless these latter also have a more general use outside the technical context. This property includes in particular identification by mathematical expressions such as coordinate systems used for the identification of instances of E53 Place. The property does not reveal anything about when, where and by whom this identifier was used. A more detailed representation can be made using the fully developed (i.e. indirect) path through E15 Identifier Assignment.

Examples:
- the capital of Italy (E53) is identified by \"Rome\" (E48)
- text 25014-32 (E33) is identified by \"The Decline and Fall of the Roman Empire\" (E35)

In First Order Logic:
P1(x,y) ⊃ E1(x)
P1(x,y) ⊃ E41(y)"@en.                          

cidoc:P1i_identifies rdfs:comment "Inverse property of 'P1_is_identified_by'."@en.


cidoc:P2_has_type
rdfs:comment "Scope note:
This property allows sub typing of CRM entities - a form of specialisation – through the use of a terminological hierarchy, or thesaurus.

The CRM is intended to focus on the high-level entities and relationships needed to describe data structures. Consequently, it does not specialise entities any further than is required for this immediate purpose. However, entities in the isA hierarchy of the CRM may by specialised into any number of sub entities, which can be defined in the E55 Type hierarchy. E51 Contact Point, for example, may be specialised into \"e-mail address\", \"telephone number\", \"post office box\", \"URL\" etc. none of which figures explicitly in the CRM hierarchy. Sub typing obviously requires consistency between the meaning of the terms assigned and the more general intent of the CRM entity in question.

Examples:
- \"enquiries@cidoc-crm.org\" (E51) has type e-mail address (E55)

In First Order Logic:
P2(x,y) ⊃ E1(x)
P2(x,y) ⊃ E55(y)"@en.
                    
cidoc:P2i_is_type_of rdfs:comment "Inverse property of 'P2_has_type'."@en.

cidoc:P3_has_note
rdfs:comment "Scope note:
This property is a container for all informal descriptions about an object that have not been expressed in terms of CRM constructs.

In particular it captures the characterisation of the item itself, its internal structures, appearance etc.
Like property P2 has type (is type of), this property is a consequence of the restricted focus of the CRM. The aim is not to capture, in a structured form, everything that can be said about an item; indeed, the CRM formalism is not regarded as sufficient to express everything that can be said. Good practice requires use of distinct note fields for different aspects of a characterisation. The P3.1 has type property of P3 has note allows differentiation of specific notes, e.g. \"construction\", \"decoration\" etc.
An item may have many notes, but a note is attached to a specific item.

Examples:
- coffee mug - OXCMS:1983.1.1 (E19) has note \"chipped at edge of handle\" (E62) has type
Condition (E55)

In First Order Logic:
P3(x,y) ⊃ E1(x)
P3(x,y) ⊃ E62(y)
P3(x,y,z) ⊃ [P3(x,y) ∧ E55(z)]

Properties: P3.1 has type: E55 Type"@en.



cidoc:P4_has_time-span rdfs:comment "This property describes the temporal confinement of an instance of an E2 Temporal Entity.
The related E52 Time-Span is understood as the real Time-Span during which the phenomena were active, which make up the temporal entity instance. It does not convey any other meaning than a positioning on the 'time-line' of chronology. The Time-Span in turn is approximated by a set of dates (E61 Time Primitive). A temporal entity can have in reality only one Time-Span, but there may exist alternative opinions about it, which we would express by assigning multiple Time-Spans. Related temporal entities may share a Time-Span. Time-Spans may have completely unknown dates but other descriptions by which we can infer knowledge."@en.

cidoc:P4i_is_time-span_of rdfs:comment "Inverse property of 'P4_has_time-span'."@en.

cidoc:P5_consists_of rdfs:comment "This property describes the decomposition of an E3 Condition State into discrete, subsidiary states. 

It is assumed that the sub-states into which the condition state is analysed form a logical whole - although the entire story may not be completely known – and that the sub-states are in fact constitutive of the general condition state. For example, a general condition state of 'in ruins' may be decomposed into the individual stages of decay.
Examples: 	
The Condition State of the ruined Parthenon (E3) consists of the bombarded state after the explosion of a Venetian shell in 1687 (E3)."@en. 

cidoc:P5i_forms_part_of rdfs:comment "Inverse property of 'P5_consists_of'."@en.

cidoc:P8_took_place_on_or_within
rdfs:comment "This property describes the location of an instance of E4 Period with respect to an E19 Physical Object.nP8 took place on or within (witnessed) is a short-cut of a path defining a E53 Place with respect to the geometry of an object. cf. E46 Section Definition.nThis property is in effect a special case of P7 took place at. It describes a period that can be located with respect to the space defined by an E19 Physical Object such as a ship or a building. The precise geographical location of the object during the period in question may be unknown or unimportant. nFor example, the French and German armistice of 22 June 1940 was signed in the same railway carriage as the armistice of 11 November 1918.n"@en.

cidoc:P8i_witnessed rdfs:comment "Inverse property of 'P8_took_place_on_or_within'."@en.

cidoc:P14_carried_out_by rdfs:comment "This property describes the active participation of an E39 Actor in an E7 Activity. 
It implies causal or legal responsibility. The P14.1 in the role of property of the property allows the nature of an Actor's participation to be specified."@en.

cidoc:P14i_performed rdfs:comment "Inverse property of 'P14_carried_out_by'."@en.

cidoc:P43_has_dimension
rdfs:comment "Scope note:
This property records a E54 Dimension of some E70 Thing.
It is a shortcut of the more fully developed path from E70 Thing through P39 measured (was measured by), E16 Measurement P40 observed dimension (was observed in) to E54 Dimension. It offers no information about how and when an E54 Dimension was established, nor by whom.

An instance of E54 Dimension is specific to an instance of E70 Thing.

Examples:
- silver cup 232 (E22) has dimension height of silver cup 232 (E54) has unit (P91) mm (E58), has value (P90) 224 (E60)

In First Order Logic:
P43(x,y) ⊃ E70(x)
P43(x,y) ⊃ E54(y)"@en.


cidoc:P43i_is_dimension_of rdfs:comment "Inverse property of 'P43_has_dimension'."@en.




cidoc:P45_consists_of
rdfs:comment "Scope note:
This property identifies the instances of E57 Materials of which an instance of E18 Physical Thing is composed.

All physical things consist of physical materials. P45 consists of (is incorporated in) allows the different Materials to be recorded. P45 consists of (is incorporated in) refers here to observed Material as opposed to the consumed raw material.

A Material, such as a theoretical alloy, may not have any physical instances.

Examples:
- silver cup 232 (E22) consists of silver (E57)

In First Order Logic:
P45(x,y) ⊃ E18(x)
P45(x,y) ⊃ E57(y)"@en.

cidoc:P45i_is_incorporated_in rdfs:comment "Inverse property of 'P45_consists_of'."@en.

cidoc:P46_is_composed_of rdfs:comment "This property allows instances of E18 Physical Thing to be analysed into component elements.
Component elements, since they are themselves instances of E18 Physical Thing, may be further analysed into sub-components, thereby creating a hierarchy of part decomposition. An instance of E18 Physical Thing may be shared between multiple wholes, for example two buildings may share a common wall.
This property is intended to describe specific components that are individually documented, rather than general aspects. Overall descriptions of the structure of an instance of E18 Physical Thing are captured by the P3 has note property.
The instances of E57 Materials of which an item of E18 Physical Thing is composed should be documented using P45 consists of (is incorporated in)."@en.


cidoc:P46i_forms_part_of
rdfs:comment "Scope note:	This property allows instances of E18 Physical Thing to be analysed into component elements.

Component elements, since they are themselves instances of E18 Physical Thing, may be further analysed into sub-components, thereby creating a hierarchy of part decomposition. An instance of E18 Physical Thing may be shared between multiple wholes, for example two buildings may share a common wall. This property does not specify when and for how long a component element resided in the respective whole. If  a component is not part of a whole from the beginning of existence or until the end of existence of the whole, the classes E79 Part Addition and E90 Part Removal can be used to document when a component became part of a particular whole and/or when it stopped being a part of it. For the time-span of being part of the respective whole, the component is completely contained in the place the whole occupies.

This property is intended to describe specific components that are individually documented, rather than general aspects. Overall descriptions of the structure of an instance of E18 Physical Thing are captured by the P3 has note property.

The instances of E57 Material of which an item of E18 Physical Thing is composed should be documented using P45 consists of (is incorporated in).
Examples: 	
	the Royal carriage (E22) forms part of the Royal train (E22)
	the 'Hog’s Back' (E24) forms part of the 'Fosseway' (E24)."@en.




cidoc:P54_has_current_permanent_location
rdfs:comment "This property records the foreseen permanent location of an instance of E19 Physical Object at the time of validity of the record or database containing the statement that uses this property.
P54 has current permanent location (is current permanent location of) is similar to P55 has current location (currently holds). However, it indicates the E53 Place currently reserved for an object, such as the permanent storage location or a permanent exhibit location. The object may be temporarily removed from the permanent location, for example when used in temporary exhibitions or loaned to another institution. The object may never actually be located at its permanent location."@en.

cidoc:P54i_is_current_permanent_location_of rdfs:comment "Inverse property of 'P54_has_current_permanent_location'."@en.

cidoc:P56_bears_feature rdfs:comment "This property describes a E26 Physical Feature found on a E19 Physical Object It does not specify the location of the feature on the object.

P56 bears feature (is found on) is a shortcut. A more detailed representation can make use of the fully developed (i.e. indirect) path from E19 Physical Object through P59 has section (is located on or within), E53 Place, P53 has former or current location (is former or current location of) to E26 Physical Feature.
A Physical Feature can only exist on one object. One object may bear more than one Physical Feature. An E27 Site should be considered as an E26 Physical Feature on the surface of the Earth.
Examples:	
	silver cup 232 (E22) bears feature 32 mm scratch on silver cup 232 (E26)
."@en.

cidoc:P56i_is_found_on rdfs:comment "Inverse property of 'P56_bears_feature'."@en.

cidoc:P67_refers_to
rdfs:comment "Scope note:
This property documents that an E89 Propositional Object makes a statement about an instance of E1 CRM Entity. P67 refers to (is referred to by) has the P67.1 has type link to an instance of E55 Type. This is intended to allow a more detailed description of the type of reference. This differs from P129 is about (is subject of), which describes the primary subject or subjects of the E89 Propositional Object.

Examples:
- the eBay auction listing for 4 July 2002 (E73) refers to silver cup 232 (E22) has type item for sale (E55)

In First Order Logic:
P67(x,y) ⊃ E89(x)
P67(x,y) ⊃ E1(y)
P67(x,y,z) ⊃ [P67(x,y) ∧ E55(z)]

Properties: P67.1 has type: E55 Type."@en.

cidoc:P67i_is_referred_by rdfs:comment "Inverse property of 'P67_refers_to'."@en.
cidoc:P68_foresees_use_of rdfs:comment "This property identifies an E57 Material foreseeen to be used by an E29 Design or Procedure. 

E29 Designs and procedures commonly foresee the use of particular E57 Materials. The fabrication of adobe bricks, for example, requires straw, clay and water. This property enables this to be documented.

This property is not intended for the documentation of E57 Materials that were used on a particular occasion when an instance of E29 Design or Procedure was executed.
Examples:	
	procedure for soda glass manufacture (E29) foresees use of soda (E57)
"@en.
cidoc:P68i_use_foreseen_by rdfs:comment "Inverse property of 'P68_foresees_use_of'."@en.

cidoc:P82_at_some_time_within
rdfs:comment "Scope note:
This property describes the maximum period of time within which an E52 Time-Span falls.

Since Time-Spans may not have precisely known temporal extents, the CRM supports statements about the minimum and maximum temporal extents of Time-Spans. This property allows a Time-Span’s maximum temporal extent (i.e. its outer boundary) to be assigned an E61 Time Primitive value. Time Primitives are treated by the CRM as application or system specific date intervals, and are not further analysed.

Examples:
- the time-span of the development of the CIDOC CRM (E52) at some time within 1992-infinity (E61)

In First Order Logic:
P82 (x,y) ⊃ E52(x)
P82 (x,y) ⊃ E61(y)"@en.


cidoc:P83_had_at_least_duration
rdfs:comment "Scope note:
This property describes the minimum length of time covered by an E52 Time-Span.

It allows an E52 Time-Span to be associated with an E54 Dimension representing it’s minimum duration (i.e. it’s inner boundary) independent from the actual beginning and end.

Examples:
- the time span of the Battle of Issos 333 B.C.E. (E52) had at least duration Battle of Issos minimum duration (E54) has unit (P91) day (E58) has value (P90) 1 (E60)

In First Order Logic:
P83(x,y) ⊃ E52(x)
P83(x,y) ⊃ E54(y)"@en.
                                  
cidoc:P83i_was_minimum_duration_of rdfs:comment "Inverse property of 'P83_had_at_least_duration'."@en.




cidoc:P84_had_at_most_duration
rdfs:comment "Scope note:
This property describes the maximum length of time covered by an E52 Time-Span.

It allows an E52 Time-Span to be associated with an E54 Dimension representing it’s maximum duration (i.e. it’s outer boundary) independent from the actual beginning and end.

Examples:
- the time span of the Battle of Issos 333 B.C.E. (E52) had at most duration Battle of Issos maximum duration (E54) has unit (P91) day (E58) has value (P90) 2 (E60)

In First Order Logic:
P84(x,y) ⊃ E52(x)
P84(x,y) ⊃ E54(y)"@en.

cidoc:P84i_was_maximum_duration_of rdfs:comment "Inverse property of 'P84_had_at_most_duration'."@en.


cidoc:P90_has_value
rdfs:comment "Scope note:
This property allows an E54 Dimension to be approximated by an E60 Number primitive.

Examples:
- height of silver cup 232 (E54) has value 226 (E60)

In First Order Logic:
P90(x,y) ⊃ E54(x)
P90(x,y) ⊃ E60(y)"@en.


cidoc:P91_has_unit
rdfs:comment "Scope note:
This property shows the type of unit an E54 Dimension was expressed in.

Examples:
- height of silver cup 232 (E54) has unit mm (E58)

In First Order Logic:
P91(x,y) ⊃ E54(x)
P91(x,y) ⊃ E58(y)"@en.

cidoc:P91i_is_unit_of rdfs:comment "Inverse property of 'P91_has_unit'."@en.


cidoc:P115_finishes rdfs:comment "This property allows the ending point for a E2 Temporal Entity to be situated by reference to the ending point of another temporal entity of longer duration.  
This property is only necessary if the time span is unknown (otherwise the relationship can be calculated). This property is the same as the 'finishes / finished-by' relationships of Allen's temporal logic (Allen, 1983, pp. 832-843)."@en.

cidoc:P115i_is_finished_by rdfs:comment "Inverse property of 'P15 finishes'."@en.

cidoc:P116_starts rdfs:comment "This property allows the starting point for a E2 Temporal Entity to be situated by reference to the starting point of another temporal entity of longer duration.  
This property is only necessary if the time span is unknown (otherwise the relationship can be calculated). This property is the same as the 'starts / started-by' relationships of Allen's temporal logic (Allen, 1983, pp. 832-843)."@en.

cidoc:P116i_is_started_by rdfs:comment "Inverse property of 'P116 starts'."@en.


cidoc:P127i_has_narrower_term rdfs:comment "Inverse property of 'cidoc:P127_has_broader_term'."@en.

cidoc:P127_has_broader_term rdfs:comment "This property identifies a super-Type to which an E55 Type is related. 
		It allows Types to be organised into hierarchies. This is the sense of 'broader term generic  		(BTG)' as defined in ISO 2788
"@en.

cidoc:P140_assigned_attribute_to rdfs:comment "This property indicates the item to which an attribute or relation is assigned. "@en.

cidoc:P140i_was_attributed_by rdfs:comment "Inverse property of 'cidoc:P140_assigned_attribute_to'."@en.

cidoc:P141_assigned
rdfs:comment "Scope note: This property indicates the attribute that was assigned or the item that was related to the item
denoted by a property P140 assigned attribute to in an Attribute assignment action.
Examples:
􀂃 February 1997 Current Ownership Assessment of Martin Doerr’s silver cup (E13)
assigned Martin Doerr (E21)
􀂃 01 June 1997 Identifier Assignment of the silver cup donated by Martin Doerr (E15)
assigned object identifier 232".


cidoc:P141i_was_assigned_by rdfs:comment "Inverse property of 'cidoc:P141_assigned'."@en.


cidoc:P148_has_component rdfs:comment "This property associates an instance of E89 Propositional Object with a structural part of it that is by itself an instance of E89 Propositional Object."@en.

cidoc:P148i_is_component_of rdfs:comment "Inverse property of 'cidoc:P148_has_component'."@en.

